isabelle-thys/Kraus_Maps.thy
@@ -426,10 +426,25 @@ lift_definition kraus_map_of_op :: \<open>('a::chilbert_space \<Rightarrow>\<^su
   is kraus_family_of_op
   by (simp add: kraus_equivalent_def)
 
+lemma sandwich_tc_scaleC_right: \<open>sandwich_tc e (c *\<^sub>C t) = c *\<^sub>C sandwich_tc e t\<close>
+  apply (transfer fixing: e c)
+  by (simp add: cblinfun.scaleC_right)
+
 lemma kraus_family_map_scaleC:
   shows \<open>kraus_family_map \<EE> (c *\<^sub>C x) = c *\<^sub>C kraus_family_map \<EE> x\<close>
-  by (simp add: kraus_family_map_def cblinfun.scaleC_right case_prod_unfold
+  by (simp add: kraus_family_map_def cblinfun.scaleC_right case_prod_unfold sandwich_tc_scaleC_right
       flip: infsum_scaleC_right)
+
+lemma sandwich_tc_plus: \<open>sandwich_tc e (t + u) = sandwich_tc e t + sandwich_tc e u\<close>
+  by (simp add: sandwich_tc_def compose_tcr.add_right compose_tcl.add_left)
+
+lemma sandwich_tc_minus: \<open>sandwich_tc e (t - u) = sandwich_tc e t - sandwich_tc e u\<close>
+  by (simp add: sandwich_tc_def compose_tcr.diff_right compose_tcl.diff_left)
+
+lemma bounded_clinear_sandwich_tc[bounded_clinear]: \<open>bounded_clinear (sandwich_tc e)\<close>
+  using norm_sandwich_tc[of e]
+  by (auto intro!: bounded_clinearI[where K=\<open>(norm e)\<^sup>2\<close>]
+      simp: sandwich_tc_plus sandwich_tc_scaleC_right cross3_simps)
 
 lemma kraus_family_map_abs_summable:
   assumes \<open>kraus_family \<EE>\<close>
@@ -446,10 +461,10 @@ proof -
       + norm (sandwich_tc x \<rho>3)
       + norm (sandwich_tc x \<rho>4)\<close> 
       (is \<open>_ \<le> ?S x\<close>) for x
-      by (auto simp add: \<rho>_decomp cblinfun.add_right cblinfun.diff_right cblinfun.scaleC_right
+      by (auto simp add: \<rho>_decomp sandwich_tc_plus sandwich_tc_minus  sandwich_tc_scaleC_right
           scaleC_add_right scaleC_diff_right norm_mult
           intro!: norm_triangle_le norm_triangle_le_diff)
-    then have *: \<open>norm (sandwich_tc (fst x) *\<^sub>V \<rho>) \<le> norm (?S (fst x))\<close> for x
+    then have *: \<open>norm (sandwich_tc (fst x) \<rho>) \<le> norm (?S (fst x))\<close> for x
       by force
     show ?thesis
       unfolding case_prod_unfold
@@ -493,18 +508,12 @@ proof -
     apply (rule nonneg_bdd_above_summable_on[rotated])
     using trace_EE\<rho>_pos 
     by (auto simp: less_eq_complex_def)
-(* 
- unfolding case_prod_unfold
-    apply (rule Infinite_Sum.summable_on_bounded_linear[rotated])
-    by (intro bounded_clinear.bounded_linear bounded_clinear_trace_duality' trace_class_from_trace_class)
-  then have \<open>(\<lambda>(E,_). trace (from_trace_class (sandwich_tc E *\<^sub>V \<rho>))) summable_on \<EE>\<close>
-    by (simp add: from_trace_class_sandwich_tc sandwich_apply circularity_of_trace trace_class_comp_right flip: cblinfun_compose_assoc)
-  *) then have \<open>(\<lambda>(E,_). Re (trace (from_trace_class (sandwich_tc E *\<^sub>V \<rho>)))) summable_on \<EE>\<close>
+ then have \<open>(\<lambda>(E,_). Re (trace (from_trace_class (sandwich_tc E \<rho>)))) summable_on \<EE>\<close>
     by (simp add: from_trace_class_sandwich_tc sandwich_apply cblinfun_assoc_right trace_class_comp_right
         flip: circularity_of_trace)
-  then have \<open>(\<lambda>(E,_). trace_norm (from_trace_class (sandwich_tc E *\<^sub>V \<rho>))) summable_on \<EE>\<close>
+  then have \<open>(\<lambda>(E,_). trace_norm (from_trace_class (sandwich_tc E \<rho>))) summable_on \<EE>\<close>
     by (simp add: aux from_trace_class_pos \<rho>_pos  sandwich_tc_pos)
-  then show \<open>(\<lambda>(E,x). sandwich_tc E *\<^sub>V \<rho>) abs_summable_on \<EE>\<close>
+  then show \<open>(\<lambda>(E,x). sandwich_tc E \<rho>) abs_summable_on \<EE>\<close>
     by (simp add: norm_trace_class.rep_eq case_prod_unfold)
 qed
 
@@ -525,14 +534,17 @@ lemma kraus_family_map_plus_right:
   shows \<open>kraus_family_map \<EE> (x + y) = kraus_family_map \<EE> x + kraus_family_map \<EE> y\<close>
   using kraus_family_map_summable[OF assms]
   by (auto intro!: infsum_add
-      simp add: kraus_family_map_def cblinfun.add_right scaleC_add_right case_prod_unfold)
+      simp add: kraus_family_map_def sandwich_tc_plus scaleC_add_right case_prod_unfold)
+
+lemma sandwich_tc_uminus_right: \<open>sandwich_tc e (- t) = - sandwich_tc e t\<close>
+  by (metis (no_types, lifting) add.right_inverse arith_simps(50) diff_0 group_cancel.sub1 sandwich_tc_minus)
 
 lemma kraus_family_map_uminus_right:
   assumes \<open>kraus_family \<EE>\<close>
   shows \<open>kraus_family_map \<EE> (- x) = - kraus_family_map \<EE> x\<close>
   using kraus_family_map_summable[OF assms]
   by (auto intro!: infsum_uminus 
-      simp add: kraus_family_map_def cblinfun.minus_right scaleC_minus_right case_prod_unfold)
+      simp add: kraus_family_map_def sandwich_tc_uminus_right scaleC_minus_right case_prod_unfold)
 
 
 lemma kraus_family_map_minus_right:
@@ -551,19 +563,19 @@ lemma kraus_family_map_bounded_pos:
   assumes \<open>kraus_family \<EE>\<close> and \<open>\<rho> \<ge> 0\<close>
   shows \<open>norm (kraus_family_map \<EE> \<rho>) \<le> kraus_family_norm \<EE> * norm \<rho>\<close>
 proof -
-  have \<open>norm (kraus_family_map \<EE> \<rho>) = Re (trace_tc (\<Sum>\<^sub>\<infinity>(E,_)\<in>\<EE>. sandwich_tc E *\<^sub>V \<rho>))\<close>
+  have \<open>norm (kraus_family_map \<EE> \<rho>) = Re (trace_tc (\<Sum>\<^sub>\<infinity>(E,_)\<in>\<EE>. sandwich_tc E \<rho>))\<close>
     apply (subst Re_complex_of_real[symmetric])
     apply (subst norm_tc_pos)
     using \<open>\<rho> \<ge> 0\<close> apply (rule kraus_family_map_pos)
     by (simp add: kraus_family_map_def case_prod_unfold)
-  also have \<open>\<dots> = (\<Sum>\<^sub>\<infinity>(E,_)\<in>\<EE>. Re (trace_tc (sandwich_tc E *\<^sub>V \<rho>)))\<close>
+  also have \<open>\<dots> = (\<Sum>\<^sub>\<infinity>(E,_)\<in>\<EE>. Re (trace_tc (sandwich_tc E \<rho>)))\<close>
     using kraus_family_map_summable[OF assms(1)]
     by (simp_all flip: infsum_bounded_linear[of \<open>\<lambda>x. Re (trace_tc x)\<close>] 
         add: case_prod_unfold bounded_linear_compose[of Re trace_tc] bounded_linear_Re
         o_def bounded_clinear.bounded_linear)
   also have \<open>\<dots> \<le> kraus_family_norm \<EE> * norm \<rho>\<close>
   proof (rule infsum_le_finite_sums)
-    show \<open>(\<lambda>(E,_). Re (trace_tc (sandwich_tc E *\<^sub>V \<rho>))) summable_on \<EE>\<close>
+    show \<open>(\<lambda>(E,_). Re (trace_tc (sandwich_tc E \<rho>))) summable_on \<EE>\<close>
       unfolding case_prod_beta
       apply (rule summable_on_bounded_linear[unfolded o_def, where h=\<open>\<lambda>x. Re (trace_tc x)\<close>])
       using kraus_family_map_summable[OF assms(1)]
@@ -571,7 +583,7 @@ proof -
         add: bounded_linear_compose[of Re trace_tc] bounded_linear_Re bounded_clinear.bounded_linear 
         o_def trace_tc_scaleC assms kraus_family_map_def case_prod_unfold)
     fix M :: \<open>(('a \<Rightarrow>\<^sub>C\<^sub>L 'b) \<times> 'c) set\<close> assume \<open>finite M\<close> and \<open>M \<subseteq> \<EE>\<close>
-    have \<open>(\<Sum>(E,_)\<in>M. Re (trace_tc (sandwich_tc E *\<^sub>V \<rho>)))
+    have \<open>(\<Sum>(E,_)\<in>M. Re (trace_tc (sandwich_tc E \<rho>)))
         = (\<Sum>(E,_)\<in>M. Re (trace (E o\<^sub>C\<^sub>L from_trace_class \<rho> o\<^sub>C\<^sub>L E*)))\<close>
       by (simp add: trace_tc.rep_eq from_trace_class_sandwich_tc sandwich_apply scaleC_trace_class.rep_eq trace_scaleC)
     also have \<open>\<dots> = (\<Sum>(E,_)\<in>M. Re (trace (E* o\<^sub>C\<^sub>L E o\<^sub>C\<^sub>L from_trace_class \<rho>)))\<close>
@@ -590,7 +602,7 @@ proof -
       apply (rule mult_right_mono)
       apply (rule kraus_family_sums_bounded_by_norm)
       using assms \<open>M \<subseteq> \<EE>\<close> by auto
-    finally show \<open>(\<Sum>(E,_)\<in>M. Re (trace_tc (sandwich_tc E *\<^sub>V \<rho>))) \<le> kraus_family_norm \<EE> * norm \<rho>\<close>
+    finally show \<open>(\<Sum>(E,_)\<in>M. Re (trace_tc (sandwich_tc E \<rho>))) \<le> kraus_family_norm \<EE> * norm \<rho>\<close>
       by -
   qed
   finally show ?thesis 
@@ -1067,7 +1079,7 @@ lemma kraus_family_map_geq_sum:
   shows \<open>kraus_family_map \<EE> \<rho> \<ge> (\<Sum>(E,_)\<in>M. sandwich_tc E \<rho>)\<close>
 proof (cases \<open>finite M\<close>)
   case True
-  have *: \<open>(\<lambda>E. sandwich_tc (fst E) *\<^sub>V \<rho>) summable_on X\<close> if \<open>X \<subseteq> \<EE>\<close> for X
+  have *: \<open>(\<lambda>E. sandwich_tc (fst E) \<rho>) summable_on X\<close> if \<open>X \<subseteq> \<EE>\<close> for X
     apply (rule summable_on_subset_banach[where A=\<EE>])
      apply (rule kraus_family_map_summable[unfolded case_prod_unfold])
     using assms that by auto
@@ -1093,27 +1105,27 @@ proof -
   have family: \<open>kraus_family (kraus_family_comp_dependent \<EE> \<FF>)\<close>
     by (auto intro!: kraus_family_kraus_family_comp_dependent assms)
 
-  have sum2: \<open>(\<lambda>(F, x). sandwich_tc F *\<^sub>V \<rho>) summable_on \<FF>\<close>
+  have sum2: \<open>(\<lambda>(F, x). sandwich_tc F \<rho>) summable_on \<FF>\<close>
     using kraus_family_map_summable[of \<FF> \<rho>] kraus\<FF> by (simp add: case_prod_unfold)
-  from family have \<open>(\<lambda>E. sandwich_tc (fst E) *\<^sub>V \<rho>) summable_on 
+  from family have \<open>(\<lambda>E. sandwich_tc (fst E) \<rho>) summable_on 
           (\<lambda>((F,y), (E,x)). (E o\<^sub>C\<^sub>L F, E, F, x, y)) ` (SIGMA (F,y):\<FF>. \<EE> y)\<close>
     using kraus_family_map_summable by (simp add: kraus_family_comp_dependent_def kraus_family_comp_def case_prod_unfold)
-  then have sum1: \<open>(\<lambda>((F,y), (E,x)). sandwich_tc (E o\<^sub>C\<^sub>L F) *\<^sub>V \<rho>) summable_on (SIGMA (F,y):\<FF>. \<EE> y)\<close>
+  then have sum1: \<open>(\<lambda>((F,y), (E,x)). sandwich_tc (E o\<^sub>C\<^sub>L F) \<rho>) summable_on (SIGMA (F,y):\<FF>. \<EE> y)\<close>
     apply (subst (asm) summable_on_reindex)
     by (auto intro!: inj_onI simp: o_def case_prod_unfold)
 
   have \<open>kraus_family_map (kraus_family_comp_dependent \<EE> \<FF>) \<rho>
-          = (\<Sum>\<^sub>\<infinity>E\<in>(\<lambda>((F,y), (E,x)). (E o\<^sub>C\<^sub>L F, E, F, x, y)) ` (SIGMA (F,y):\<FF>. \<EE> y). sandwich_tc (fst E) *\<^sub>V \<rho>)\<close>
+          = (\<Sum>\<^sub>\<infinity>E\<in>(\<lambda>((F,y), (E,x)). (E o\<^sub>C\<^sub>L F, E, F, x, y)) ` (SIGMA (F,y):\<FF>. \<EE> y). sandwich_tc (fst E) \<rho>)\<close>
     by (simp add: kraus_family_map_def kraus_family_comp_dependent_def kraus_family_comp_def case_prod_unfold)
-  also have \<open>\<dots> = (\<Sum>\<^sub>\<infinity>((F,y), (E,x))\<in>(SIGMA (F,y):\<FF>. \<EE> y). sandwich_tc (E o\<^sub>C\<^sub>L F) *\<^sub>V \<rho>)\<close>
+  also have \<open>\<dots> = (\<Sum>\<^sub>\<infinity>((F,y), (E,x))\<in>(SIGMA (F,y):\<FF>. \<EE> y). sandwich_tc (E o\<^sub>C\<^sub>L F) \<rho>)\<close>
     apply (subst infsum_reindex)
     by (auto intro!: inj_onI simp: o_def case_prod_unfold)
-  also have \<open>\<dots> = (\<Sum>\<^sub>\<infinity>(F,y)\<in>\<FF>. \<Sum>\<^sub>\<infinity>(E,x)\<in>\<EE> y. sandwich_tc (E o\<^sub>C\<^sub>L F) *\<^sub>V \<rho>)\<close>
+  also have \<open>\<dots> = (\<Sum>\<^sub>\<infinity>(F,y)\<in>\<FF>. \<Sum>\<^sub>\<infinity>(E,x)\<in>\<EE> y. sandwich_tc (E o\<^sub>C\<^sub>L F) \<rho>)\<close>
     apply (subst infsum_Sigma'_banach[symmetric])
     using sum1 by (auto simp: case_prod_unfold)
-  also have \<open>\<dots> = (\<Sum>\<^sub>\<infinity>(F,y)\<in>\<FF>. \<Sum>\<^sub>\<infinity>(E,x)\<in>\<EE> y. sandwich_tc E *\<^sub>V sandwich_tc F *\<^sub>V \<rho>)\<close>
+  also have \<open>\<dots> = (\<Sum>\<^sub>\<infinity>(F,y)\<in>\<FF>. \<Sum>\<^sub>\<infinity>(E,x)\<in>\<EE> y. sandwich_tc E (sandwich_tc F \<rho>))\<close>
     by (simp add: sandwich_tc_compose)
-  also have \<open>\<dots> = (\<Sum>\<^sub>\<infinity>(F,y)\<in>\<FF>. kraus_family_map (\<EE> y) (sandwich_tc F *\<^sub>V \<rho>))\<close>
+  also have \<open>\<dots> = (\<Sum>\<^sub>\<infinity>(F,y)\<in>\<FF>. kraus_family_map (\<EE> y) (sandwich_tc F \<rho>))\<close>
     by (simp add: kraus_family_map_def case_prod_unfold)
   finally show ?thesis
     by -
@@ -1128,7 +1140,7 @@ proof (rule ext, rename_tac \<rho>)
   fix \<rho> :: \<open>('c, 'c) trace_class\<close>
 
   from \<open>kraus_family \<FF>\<close>
-  have sumF: \<open>(\<lambda>(F, y). sandwich_tc F *\<^sub>V \<rho>) summable_on \<FF>\<close>
+  have sumF: \<open>(\<lambda>(F, y). sandwich_tc F \<rho>) summable_on \<FF>\<close>
     by (rule kraus_family_map_summable)
   have \<open>kraus_family_map (kraus_family_comp \<EE> \<FF>) \<rho> = (\<Sum>\<^sub>\<infinity>(F,y)\<in>\<FF>. kraus_family_map \<EE> (sandwich_tc F \<rho>))\<close>
     by (auto intro!: kraus_family_comp_dependent_apply simp: kraus_family_comp_def \<open>kraus_family \<EE>\<close> \<open>kraus_family \<FF>\<close>)
@@ -1423,40 +1435,40 @@ proof (rule ext)
   show \<open>kraus_family_map (kraus_family_flatten \<EE>) \<rho> = \<sigma>\<close>
   proof -
     from \<open>kraus_family \<EE>\<close>
-    have \<open>(\<lambda>(F,x). sandwich_tc F *\<^sub>V \<rho>) summable_on \<EE>\<close>
+    have \<open>(\<lambda>(F,x). sandwich_tc F \<rho>) summable_on \<EE>\<close>
       using kraus_family_map_summable by (simp add: case_prod_unfold)
-    then have \<open>((\<lambda>(F,x). sandwich_tc F *\<^sub>V \<rho>) has_sum \<sigma>) \<EE>\<close>
+    then have \<open>((\<lambda>(F,x). sandwich_tc F \<rho>) has_sum \<sigma>) \<EE>\<close>
       by (simp add: \<sigma>_def kraus_family_map_def split_def)
-    then have \<open>((\<lambda>(F,x). sandwich_tc F *\<^sub>V \<rho>) has_sum \<sigma>) {(F,x)\<in>\<EE>. F \<noteq> 0}\<close>
+    then have \<open>((\<lambda>(F,x). sandwich_tc F \<rho>) has_sum \<sigma>) {(F,x)\<in>\<EE>. F \<noteq> 0}\<close>
       apply (rule has_sum_cong_neutral[THEN iffD2, rotated -1])
       by auto
-    then have \<open>((\<lambda>(F,x). sandwich_tc F *\<^sub>V \<rho>) has_sum \<sigma>)
+    then have \<open>((\<lambda>(F,x). sandwich_tc F \<rho>) has_sum \<sigma>)
            (snd ` (SIGMA (E,x::unit):{E. good (fst E)}. kraus_family_related_ops \<EE> E))\<close>
       by (simp add: snd_sigma)
-    then have \<open>((\<lambda>((E,x::unit), (F,y)). sandwich_tc F *\<^sub>V \<rho>) has_sum \<sigma>)
+    then have \<open>((\<lambda>((E,x::unit), (F,y)). sandwich_tc F \<rho>) has_sum \<sigma>)
        (SIGMA (E,x):{E. good (fst E)}. kraus_family_related_ops \<EE> E)\<close>
       apply (subst (asm) has_sum_reindex)
       by (auto intro!: inj_on_def inj_snd simp: o_def case_prod_unfold)
-    then have sum1: \<open>((\<lambda>((E,x::unit), (F,x)). (norm F)\<^sup>2 *\<^sub>R sandwich_tc (normal E) *\<^sub>V \<rho>) has_sum \<sigma>)
+    then have sum1: \<open>((\<lambda>((E,x::unit), (F,x)). (norm F)\<^sup>2 *\<^sub>R sandwich_tc (normal E) \<rho>) has_sum \<sigma>)
     (SIGMA (E,x):{p. good (fst p)}. kraus_family_related_ops \<EE> E)\<close>
       apply (rule has_sum_cong[THEN iffD2, rotated])
       apply (auto intro!: simp: good_def normal_def sandwich_tc_scaleR_left power_inverse real_sqrt_pow2 E_inv
           kraus_family_related_ops_def kraus_family_op_weight_scale)
       by (metis (no_types, opaque_lifting) Extra_Ordered_Fields.sign_simps(5) linorder_not_less more_arith_simps(11) mult_eq_0_iff norm_le_zero_iff order.refl power2_eq_square right_inverse scale_one)
     then have \<open>((\<lambda>(E,_). \<Sum>\<^sub>\<infinity>(F, x)\<in>kraus_family_related_ops \<EE> E.
-                (norm F)\<^sup>2 *\<^sub>R sandwich_tc (normal E) *\<^sub>V \<rho>) has_sum \<sigma>) {(E, x::unit). good E}\<close>
+                (norm F)\<^sup>2 *\<^sub>R sandwich_tc (normal E) \<rho>) has_sum \<sigma>) {(E, x::unit). good E}\<close>
       by (auto intro!: has_sum_Sigma'_banach simp add: case_prod_unfold)
-    then have \<open>((\<lambda>(E,_). (\<Sum>\<^sub>\<infinity>(F, x)\<in>kraus_family_related_ops \<EE> E. (norm F)\<^sup>2) *\<^sub>R sandwich_tc (normal E) *\<^sub>V \<rho>)
+    then have \<open>((\<lambda>(E,_). (\<Sum>\<^sub>\<infinity>(F, x)\<in>kraus_family_related_ops \<EE> E. (norm F)\<^sup>2) *\<^sub>R sandwich_tc (normal E) \<rho>)
                         has_sum \<sigma>) {(E, x::unit). good E}\<close>
       apply (rule has_sum_cong[THEN iffD1, rotated])
       apply auto
       by (smt (verit) Complex_Vector_Spaces.infsum_scaleR_left cblinfun.scaleR_left infsum_cong split_def)
-    then have \<open>((\<lambda>(E,_). kraus_family_op_weight \<EE> E *\<^sub>R sandwich_tc (normal E) *\<^sub>V \<rho>) has_sum \<sigma>) {(E, x::unit). good E}\<close>
+    then have \<open>((\<lambda>(E,_). kraus_family_op_weight \<EE> E *\<^sub>R sandwich_tc (normal E) \<rho>) has_sum \<sigma>) {(E, x::unit). good E}\<close>
       by (simp add: kraus_family_op_weight_def)
-    then have \<open>((\<lambda>(E,_). sandwich_tc E *\<^sub>V \<rho>) has_sum \<sigma>) {(E, x::unit). good E}\<close>
+    then have \<open>((\<lambda>(E,_). sandwich_tc E \<rho>) has_sum \<sigma>) {(E, x::unit). good E}\<close>
       apply (rule has_sum_cong[THEN iffD1, rotated])
       by (auto intro!: simp: normal_def sandwich_tc_scaleR_left power_inverse real_sqrt_pow2 E_inv)
-    then have \<open>((\<lambda>(E,_). sandwich_tc E *\<^sub>V \<rho>) has_sum \<sigma>) (kraus_family_flatten \<EE>)\<close>
+    then have \<open>((\<lambda>(E,_). sandwich_tc E \<rho>) has_sum \<sigma>) (kraus_family_flatten \<EE>)\<close>
       by (simp add: kraus_family_flatten_def good_def)
     then show \<open>kraus_family_map (kraus_family_flatten \<EE>) \<rho> = \<sigma>\<close>
       by (simp add: kraus_family_map_def case_prod_unfold infsumI)
@@ -1558,15 +1570,15 @@ lemma kraus_family_map_plus:
   shows \<open>kraus_family_map (kraus_family_plus \<EE> \<FF>) \<rho> = kraus_family_map \<EE> \<rho> + kraus_family_map \<FF> \<rho>\<close>
 proof -
   have \<open>kraus_family_map (kraus_family_plus \<EE> \<FF>) \<rho> = 
-    (\<Sum>\<^sub>\<infinity>EF\<in>(\<lambda>(E,x). (E, Inl x)) ` \<EE> \<union> (\<lambda>(F,y). (F, Inr y)) ` \<FF>. sandwich_tc (fst EF) *\<^sub>V \<rho>)\<close>
+    (\<Sum>\<^sub>\<infinity>EF\<in>(\<lambda>(E,x). (E, Inl x)) ` \<EE> \<union> (\<lambda>(F,y). (F, Inr y)) ` \<FF>. sandwich_tc (fst EF) \<rho>)\<close>
     by (simp add: kraus_family_plus_def kraus_family_map_def case_prod_unfold)
-  also have \<open>\<dots> = (\<Sum>\<^sub>\<infinity>EF\<in>(\<lambda>(E,x). (E, Inl x :: 'x+'y)) ` \<EE>. sandwich_tc (fst EF) *\<^sub>V \<rho>)
-                + (\<Sum>\<^sub>\<infinity>EF\<in>(\<lambda>(F,y). (F, Inr y :: 'x+'y)) ` \<FF>. sandwich_tc (fst EF) *\<^sub>V \<rho>)\<close>
+  also have \<open>\<dots> = (\<Sum>\<^sub>\<infinity>EF\<in>(\<lambda>(E,x). (E, Inl x :: 'x+'y)) ` \<EE>. sandwich_tc (fst EF) \<rho>)
+                + (\<Sum>\<^sub>\<infinity>EF\<in>(\<lambda>(F,y). (F, Inr y :: 'x+'y)) ` \<FF>. sandwich_tc (fst EF) \<rho>)\<close>
     apply (subst infsum_Un_disjoint)
     using assms kraus_family_map_summable
     by (auto intro!: summable_on_reindex[THEN iffD2] inj_onI
         simp: o_def case_prod_unfold kraus_family_map_summable)
-  also have \<open>\<dots> = (\<Sum>\<^sub>\<infinity>E\<in>\<EE>. sandwich_tc (fst E) *\<^sub>V \<rho>) + (\<Sum>\<^sub>\<infinity>F\<in>\<FF>. sandwich_tc (fst F) *\<^sub>V \<rho>)\<close>
+  also have \<open>\<dots> = (\<Sum>\<^sub>\<infinity>E\<in>\<EE>. sandwich_tc (fst E) \<rho>) + (\<Sum>\<^sub>\<infinity>F\<in>\<FF>. sandwich_tc (fst F) \<rho>)\<close>
     apply (subst infsum_reindex)
      apply (auto intro!: inj_onI)[1]
     apply (subst infsum_reindex)
@@ -1685,11 +1697,11 @@ lift_definition kraus_map_apply :: \<open>('a::chilbert_space,'b::chilbert_space
   \<open>kraus_family_map\<close>
   by (auto simp: kraus_equivalent_def kraus_family_map_bounded_clinear)
 
-lemma kraus_family_of_op_apply: \<open>kraus_family_map (kraus_family_of_op E) \<rho> = sandwich_tc E *\<^sub>V \<rho>\<close>
+lemma kraus_family_of_op_apply: \<open>kraus_family_map (kraus_family_of_op E) \<rho> = sandwich_tc E \<rho>\<close>
   by (simp add: kraus_family_map_def kraus_family_of_op_def)
 
 
-lemma kraus_map_of_op_apply: \<open>kraus_map_apply (kraus_map_of_op E) \<rho> = sandwich_tc E *\<^sub>V \<rho>\<close>
+lemma kraus_map_of_op_apply: \<open>kraus_map_apply (kraus_map_of_op E) \<rho> = sandwich_tc E \<rho>\<close>
   apply (transfer' fixing: \<rho>)
   by (simp add: kraus_family_of_op_apply)
 
@@ -1902,12 +1914,12 @@ lemma norm_tc_tensor: \<open>norm (tc_tensor a b) = norm a * norm b\<close>
   shows \<open>(rel_set cr_trace_class ===> rel_set cr_trace_class) cspan cspan\<close>
   by - *)
 
-definition trace_kraus_family :: \<open>'a set \<Rightarrow> ('a::chilbert_space, complex, 'a) kraus_family\<close> where
+definition trace_kraus_family :: \<open>'a set \<Rightarrow> ('a::chilbert_space, 'b::one_dim, 'a) kraus_family\<close> where
   \<open>trace_kraus_family B = (\<lambda>x. (vector_to_cblinfun x*, x)) ` B\<close>
 
 lemma trace_kraus_family_is_kraus_family: \<open>kraus_family (trace_kraus_family B)\<close> if \<open>is_onb B\<close>
 proof -
-  have \<open>(\<Sum>(E, x)\<in>F. E* o\<^sub>C\<^sub>L E) \<le> id_cblinfun\<close> if \<open>finite F\<close> and FB: \<open>F \<subseteq> trace_kraus_family B\<close> for F :: \<open>('a \<Rightarrow>\<^sub>C\<^sub>L complex \<times> 'a) set\<close>
+  have \<open>(\<Sum>(E, x)\<in>F. E* o\<^sub>C\<^sub>L E) \<le> id_cblinfun\<close> if \<open>finite F\<close> and FB: \<open>F \<subseteq> trace_kraus_family B\<close> for F :: \<open>('a \<Rightarrow>\<^sub>C\<^sub>L 'b \<times> 'a) set\<close>
   proof -
     obtain G where \<open>finite G\<close> and \<open>G \<subseteq> B\<close> and FG: \<open>F = (\<lambda>x. (vector_to_cblinfun x*, x)) ` G\<close>
       apply atomize_elim
@@ -1921,7 +1933,7 @@ proof -
     have [simp]: \<open>inj_on (\<lambda>x. (vector_to_cblinfun x*, x)) G\<close>
       by (meson inj_onI prod.inject)
     have \<open>(\<Sum>(E, x)\<in>F. E* o\<^sub>C\<^sub>L E) = (\<Sum>x\<in>G. selfbutter x)\<close>
-      by (simp add: FG sum.reindex butterfly_def)
+      by (simp add: FG sum.reindex flip: butterfly_def_one_dim)
     also have \<open>(\<Sum>x\<in>G. selfbutter x) \<le> id_cblinfun\<close>
       apply (rule sum_butterfly_leq_id)
       by auto
@@ -1938,7 +1950,7 @@ lemma trace_kraus_family_is_trace:
   shows \<open>kraus_family_map (trace_kraus_family B) \<rho> = one_dim_iso (trace_tc \<rho>)\<close>
 proof -
   define \<rho>' where \<open>\<rho>' = from_trace_class \<rho>\<close>
-  have \<open>kraus_family_map (trace_kraus_family B) \<rho> = (\<Sum>\<^sub>\<infinity>x\<in>B. sandwich_tc (vector_to_cblinfun x*) *\<^sub>V \<rho>)\<close>
+  have \<open>kraus_family_map (trace_kraus_family B) \<rho> = (\<Sum>\<^sub>\<infinity>x\<in>B. sandwich_tc (vector_to_cblinfun x*) \<rho>)\<close>
     apply (simp add: kraus_family_map_def trace_kraus_family_def)
     apply (subst infsum_reindex)
      apply (meson inj_onI prod.simps(1))
@@ -1964,7 +1976,7 @@ lemma kraus_equivalent_trace_kraus_family:
       simp: kraus_equivalent_def trace_kraus_family_is_trace assms)
 
 
-lift_definition trace_kraus_map :: \<open>('a::chilbert_space, complex) kraus_map\<close> is
+lift_definition trace_kraus_map :: \<open>('a::chilbert_space, 'b::one_dim) kraus_map\<close> is
   \<open>kraus_family_flatten (trace_kraus_family some_chilbert_basis)\<close>
   by (simp add: kraus_equivalent_reflI kraus_family_kraus_family_flatten trace_kraus_family_is_kraus_family)
 
@@ -2002,51 +2014,826 @@ lemma kraus_equivalent_trans[trans]:
   \<open>kraus_equivalent F G \<Longrightarrow> kraus_equivalent G H \<Longrightarrow> kraus_equivalent F H\<close>
   by (simp add: kraus_equivalent_def)
 
-definition kraus_family_tensor :: \<open>('a ell2, 'b ell2, 'x) kraus_family \<Rightarrow> ('c ell2, 'd ell2, 'y) kraus_family \<Rightarrow> (('a\<times>'c) ell2, ('b\<times>'d) ell2, ('x\<times>'y)) kraus_family\<close> where
-  \<open>kraus_family_tensor \<EE> \<FF> = (\<lambda>((E,x), (F,y)). (E \<otimes>\<^sub>o F, (x,y))) ` (\<EE>\<times>\<FF>)\<close>
+definition kraus_family_tensor :: \<open>('a ell2, 'b ell2, 'x) kraus_family \<Rightarrow> ('c ell2, 'd ell2, 'y) kraus_family \<Rightarrow> (('a\<times>'c) ell2, ('b\<times>'d) ell2, (_\<times>_\<times>'x\<times>'y)) kraus_family\<close> where
+  \<open>kraus_family_tensor \<EE> \<FF> = (\<lambda>((E,x), (F,y)). (E \<otimes>\<^sub>o F, (E,F,x,y))) ` (\<EE>\<times>\<FF>)\<close>
+
+lemma tc_butterfly_add_left: \<open>tc_butterfly (a + a') b = tc_butterfly a b + tc_butterfly a' b\<close>
+  apply transfer
+  by (rule butterfly_add_left)
+
+lemma tc_butterfly_add_right: \<open>tc_butterfly a (b + b') = tc_butterfly a b + tc_butterfly a b'\<close>
+  apply transfer
+  by (rule butterfly_add_right)
+
+lemma tc_butterfly_sum_left: \<open>tc_butterfly (\<Sum>i\<in>M. \<psi> i) \<phi> = (\<Sum>i\<in>M. tc_butterfly (\<psi> i) \<phi>)\<close>
+  apply transfer
+  by (rule butterfly_sum_left)
+
+lemma tc_butterfly_sum_right: \<open>tc_butterfly \<psi> (\<Sum>i\<in>M. \<phi> i) = (\<Sum>i\<in>M. tc_butterfly \<psi> (\<phi> i))\<close>
+  apply transfer
+  by (rule butterfly_sum_right)
+
+lemma tc_butterfly_scaleC_left[simp]: "tc_butterfly (c *\<^sub>C \<psi>) \<phi> = c *\<^sub>C tc_butterfly \<psi> \<phi>"
+  apply transfer by simp
+
+lemma tc_butterfly_scaleC_right[simp]: "tc_butterfly \<psi> (c *\<^sub>C \<phi>) = cnj c *\<^sub>C tc_butterfly \<psi> \<phi>"
+  apply transfer by simp
+
+lemma onb_butterflies_span_trace_class:
+  fixes A :: \<open>'a::chilbert_space set\<close> and B :: \<open>'b::chilbert_space set\<close>
+  assumes \<open>is_onb A\<close> and \<open>is_onb B\<close>
+  shows \<open>ccspan ((\<lambda>(x, y). tc_butterfly x y) ` (A\<times>B)) = \<top>\<close>
+proof -
+  have \<open>closure (cspan ((\<lambda>(x, y). tc_butterfly x y) ` (A\<times>B))) \<supseteq> Collect rank1_tc\<close>
+  proof (rule subsetI)
+    \<comment> \<open>This subproof is almost identical to the corresponding one in
+        @{thm [source] finite_rank_dense_compact}, and lengthy. Can they be merged into one subproof?\<close>
+    fix x :: \<open>('b, 'a) trace_class\<close> assume \<open>x \<in> Collect rank1_tc\<close>
+    then obtain a b where xab: \<open>x = tc_butterfly a b\<close>
+      apply transfer using rank1_iff_butterfly by fastforce
+    define f where \<open>f F G = tc_butterfly (Proj (ccspan F) a) (Proj (ccspan G) b)\<close> for F G
+    have lim: \<open>(case_prod f \<longlongrightarrow> x) (finite_subsets_at_top A \<times>\<^sub>F finite_subsets_at_top B)\<close>
+    proof (rule tendstoI, subst dist_norm)
+      fix e :: real assume \<open>e > 0\<close>
+      define d where \<open>d = (if norm a = 0 \<and> norm b = 0 then 1 
+                                  else e / (max (norm a) (norm b)) / 4)\<close>
+      have d: \<open>norm a * d + norm a * d + norm b * d < e\<close>
+      proof -
+        have \<open>norm a * d \<le> e/4\<close>
+          using \<open>e > 0\<close> apply (auto simp: d_def)
+           apply (simp add: divide_le_eq)
+          by (smt (z3) Extra_Ordered_Fields.mult_sign_intros(3) \<open>0 < e\<close> antisym_conv divide_le_eq less_imp_le linordered_field_class.mult_imp_div_pos_le mult_left_mono nice_ordered_field_class.dense_le nice_ordered_field_class.divide_nonneg_neg nice_ordered_field_class.divide_nonpos_pos nle_le nonzero_mult_div_cancel_left norm_imp_pos_and_ge ordered_field_class.sign_simps(5) split_mult_pos_le)
+        moreover have \<open>norm b * d \<le> e/4\<close>
+          using \<open>e > 0\<close> apply (auto simp: d_def)
+           apply (simp add: divide_le_eq)
+          by (smt (verit) linordered_field_class.mult_imp_div_pos_le mult_left_mono norm_le_zero_iff ordered_field_class.sign_simps(5))
+        ultimately have \<open>norm a * d + norm a * d + norm b * d \<le> 3 * e / 4\<close>
+          by linarith
+        also have \<open>\<dots> < e\<close>
+          by (simp add: \<open>0 < e\<close>)
+        finally show ?thesis
+          by -
+      qed
+      have [simp]: \<open>d > 0\<close>
+        using \<open>e > 0\<close> apply (auto simp: d_def)
+         apply (smt (verit, best) nice_ordered_field_class.divide_pos_pos norm_eq_zero norm_not_less_zero)
+        by (smt (verit) linordered_field_class.divide_pos_pos zero_less_norm_iff)
+      from Proj_onb_limit[where \<psi>=a, OF assms(1)]
+      have \<open>\<forall>\<^sub>F F in finite_subsets_at_top A. norm (Proj (ccspan F) a - a) < d\<close>
+        by (metis Lim_null \<open>0 < d\<close> order_tendstoD(2) tendsto_norm_zero_iff)
+      moreover from Proj_onb_limit[where \<psi>=b, OF assms(2)]
+      have \<open>\<forall>\<^sub>F G in finite_subsets_at_top B. norm (Proj (ccspan G) b - b) < d\<close>
+        by (metis Lim_null \<open>0 < d\<close> order_tendstoD(2) tendsto_norm_zero_iff)
+      ultimately have FG_close: \<open>\<forall>\<^sub>F (F,G) in finite_subsets_at_top A \<times>\<^sub>F finite_subsets_at_top B. 
+              norm (Proj (ccspan F) a - a) < d \<and> norm (Proj (ccspan G) b - b) < d\<close>
+        unfolding case_prod_beta
+        by (rule eventually_prodI)
+      have fFG_dist: \<open>norm (f F G - x) < e\<close> 
+        if \<open>norm (Proj (ccspan F) a - a) < d\<close> and \<open>norm (Proj (ccspan G) b - b) < d\<close>
+          and \<open>F \<subseteq> A\<close> and \<open>G \<subseteq> B\<close> for F G
+      proof -
+        have a_split: \<open>a = Proj (ccspan F) a + Proj (ccspan (A-F)) a\<close>
+          using assms apply (simp add: is_onb_def is_ortho_set_def that Proj_orthog_ccspan_union flip: cblinfun.add_left)
+          apply (subst Proj_orthog_ccspan_union[symmetric])
+           apply (metis DiffD1 DiffD2 in_mono that(3))
+          using \<open>F \<subseteq> A\<close> by (auto intro!: simp: Un_absorb1)
+        have b_split: \<open>b = Proj (ccspan G) b + Proj (ccspan (B-G)) b\<close>
+          using assms apply (simp add: is_onb_def is_ortho_set_def that Proj_orthog_ccspan_union flip: cblinfun.add_left)
+          apply (subst Proj_orthog_ccspan_union[symmetric])
+           apply (metis DiffD1 DiffD2 in_mono that(4))
+          using \<open>G \<subseteq> B\<close> by (auto intro!: simp: Un_absorb1)
+        have n1: \<open>norm (f F (B-G)) \<le> norm a * d\<close> for F
+        proof -
+          have \<open>norm (f F (B-G)) \<le> norm a * norm (Proj (ccspan (B-G)) b)\<close>
+            by (auto intro!: mult_right_mono is_Proj_reduces_norm simp add: f_def norm_tc_butterfly)
+          also have \<open>\<dots> \<le> norm a * norm (Proj (ccspan G) b - b)\<close>
+            by (metis add_diff_cancel_left' b_split less_eq_real_def norm_minus_commute)
+          also have \<open>\<dots> \<le> norm a * d\<close>
+            by (meson less_eq_real_def mult_left_mono norm_ge_zero that(2))
+          finally show ?thesis
+            by -
+        qed
+        have n2: \<open>norm (f (A-F) G) \<le> norm b * d\<close> for G
+        proof -
+          have \<open>norm (f (A-F) G) \<le> norm b * norm (Proj (ccspan (A-F)) a)\<close>
+            by (auto intro!: mult_right_mono is_Proj_reduces_norm simp add: f_def norm_tc_butterfly mult.commute)
+          also have \<open>\<dots> \<le> norm b * norm (Proj (ccspan F) a - a)\<close>
+            by (smt (verit, best) a_split add_diff_cancel_left' minus_diff_eq norm_minus_cancel)
+          also have \<open>\<dots> \<le> norm b * d\<close>
+            by (meson less_eq_real_def mult_left_mono norm_ge_zero that(1))
+          finally show ?thesis
+            by -
+        qed
+        have \<open>norm (f F G - x) = norm (- f F (B-G) - f (A-F) (B-G) - f (A-F) G)\<close>
+          unfolding xab
+          apply (subst a_split, subst b_split)
+          by (simp add: f_def tc_butterfly_add_right tc_butterfly_add_left)
+        also have \<open>\<dots> \<le> norm (f F (B-G)) + norm (f (A-F) (B-G)) + norm (f (A-F) G)\<close>
+          by (smt (verit, best) norm_minus_cancel norm_triangle_ineq4)
+        also have \<open>\<dots> \<le> norm a * d + norm a * d + norm b * d\<close>
+          using n1 n2
+          by (meson add_mono_thms_linordered_semiring(1))
+        also have \<open>\<dots> < e\<close>
+          by (fact d)
+        finally show ?thesis
+          by -
+      qed
+      show \<open>\<forall>\<^sub>F FG in finite_subsets_at_top A \<times>\<^sub>F finite_subsets_at_top B. norm (case_prod f FG - x) < e\<close>
+        apply (rule eventually_elim2)
+          apply (rule eventually_prodI[where P=\<open>\<lambda>F. finite F \<and> F \<subseteq> A\<close> and Q=\<open>\<lambda>G. finite G \<and> G \<subseteq> B\<close>])
+           apply auto[2]
+         apply (rule FG_close)
+        using fFG_dist by fastforce
+    qed
+    have nontriv: \<open>finite_subsets_at_top A \<times>\<^sub>F finite_subsets_at_top B \<noteq> \<bottom>\<close>
+      by (simp add: prod_filter_eq_bot)
+    have inside: \<open>\<forall>\<^sub>F x in finite_subsets_at_top A \<times>\<^sub>F finite_subsets_at_top B. 
+              case_prod f x \<in> cspan ((\<lambda>(\<xi>,\<eta>). tc_butterfly \<xi> \<eta>) ` (A \<times> B))\<close>
+    proof (rule eventually_mp[where P=\<open>\<lambda>(F,G). finite F \<and> finite G\<close>])
+      show \<open>\<forall>\<^sub>F (F,G) in finite_subsets_at_top A \<times>\<^sub>F finite_subsets_at_top B. finite F \<and> finite G\<close>
+        by (smt (verit) case_prod_conv eventually_finite_subsets_at_top_weakI eventually_prod_filter)
+      have f_in_span: \<open>f F G \<in> cspan ((\<lambda>(\<xi>,\<eta>). tc_butterfly \<xi> \<eta>) ` (A \<times> B))\<close> if [simp]: \<open>finite F\<close> \<open>finite G\<close> and \<open>F \<subseteq> A\<close> \<open>G \<subseteq> B\<close> for F G
+      proof -
+        have \<open>Proj (ccspan F) a \<in> cspan F\<close>
+          by (metis Proj_range cblinfun_apply_in_image ccspan_finite that(1))
+        then obtain r where ProjFsum: \<open>Proj (ccspan F) a = (\<Sum>x\<in>F. r x *\<^sub>C x)\<close>
+          apply atomize_elim
+          using complex_vector.span_finite[OF \<open>finite F\<close>]
+          by auto
+        have \<open>Proj (ccspan G) b \<in> cspan G\<close>
+          by (metis Proj_range cblinfun_apply_in_image ccspan_finite that(2))
+        then obtain s where ProjGsum: \<open>Proj (ccspan G) b = (\<Sum>x\<in>G. s x *\<^sub>C x)\<close>
+          apply atomize_elim
+          using complex_vector.span_finite[OF \<open>finite G\<close>]
+          by auto
+        have \<open>tc_butterfly \<xi> \<eta> \<in> (\<lambda>(\<xi>, \<eta>). tc_butterfly \<xi> \<eta>) ` (A \<times> B)\<close>
+          if \<open>\<eta> \<in> G\<close> and \<open>\<xi> \<in> F\<close> for \<eta> \<xi>
+          using \<open>F \<subseteq> A\<close> \<open>G \<subseteq> B\<close> that by (auto intro!: pair_imageI)
+        then show ?thesis
+          by (auto intro!: complex_vector.span_sum complex_vector.span_scale
+              intro: complex_vector.span_base[where a=\<open>tc_butterfly _ _\<close>]
+              simp add: f_def ProjFsum ProjGsum tc_butterfly_sum_left tc_butterfly_sum_right)
+      qed
+      show \<open>\<forall>\<^sub>F x in finite_subsets_at_top A \<times>\<^sub>F finite_subsets_at_top B.
+                      (case x of (F, G) \<Rightarrow> finite F \<and> finite G) \<longrightarrow> (case x of (F, G) \<Rightarrow> f F G) \<in> cspan ((\<lambda>(\<xi>, \<eta>). tc_butterfly \<xi> \<eta>) ` (A \<times> B))\<close>
+        apply (rule eventually_mono)
+        apply (rule eventually_prodI[where P=\<open>\<lambda>F. finite F \<and> F \<subseteq> A\<close> and Q=\<open>\<lambda>G. finite G \<and> G \<subseteq> B\<close>])
+        by (auto intro!: f_in_span)
+    qed
+    show \<open>x \<in> closure (cspan ((\<lambda>(\<xi>, \<eta>). tc_butterfly \<xi> \<eta>) ` (A \<times> B)))\<close>
+      using lim nontriv inside by (rule limit_in_closure)
+  qed
+  moreover have \<open>cspan (Collect rank1_tc :: ('b,'a) trace_class set) = Collect finite_rank_tc\<close>
+    using finite_rank_tc_def' by fastforce
+  moreover have \<open>closure (Collect finite_rank_tc :: ('b,'a) trace_class set) = UNIV\<close>
+    by (rule finite_rank_tc_dense)
+  ultimately have \<open>closure (cspan ((\<lambda>(x, y). tc_butterfly x y) ` (A\<times>B))) \<supseteq> UNIV\<close>
+    by (smt (verit, del_insts) Un_UNIV_left closed_sum_closure_left closed_sum_cspan closure_closure closure_is_csubspace complex_vector.span_eq_iff complex_vector.subspace_span subset_Un_eq)
+  then show ?thesis
+    by (metis ccspan.abs_eq ccspan_UNIV closure_UNIV complex_vector.span_UNIV top.extremum_uniqueI)
+qed
+
+
+lemma tensor_op_mono_left:
+  fixes a :: \<open>'a ell2 \<Rightarrow>\<^sub>C\<^sub>L 'a ell2\<close> and c :: \<open>'b ell2 \<Rightarrow>\<^sub>C\<^sub>L 'b ell2\<close>
+  assumes \<open>a \<le> b\<close> and \<open>c \<ge> 0\<close>
+  shows \<open>a \<otimes>\<^sub>o c \<le> b \<otimes>\<^sub>o c\<close>
+proof -
+  have \<open>b - a \<ge> 0\<close>
+    by (simp add: assms(1))
+  with \<open>c \<ge> 0\<close> have \<open>(b - a) \<otimes>\<^sub>o c \<ge> 0\<close>
+    by (intro tensor_op_pos)
+  then have \<open>b \<otimes>\<^sub>o c - a \<otimes>\<^sub>o c \<ge> 0\<close>
+    by (simp add: tensor_op_cbilinear.diff_left)
+  then show ?thesis
+    by simp
+qed
+
+lemma tensor_op_mono_right:
+  fixes a :: \<open>'a ell2 \<Rightarrow>\<^sub>C\<^sub>L 'a ell2\<close> and b :: \<open>'b ell2 \<Rightarrow>\<^sub>C\<^sub>L 'b ell2\<close>
+  assumes \<open>b \<le> c\<close> and \<open>a \<ge> 0\<close>
+  shows \<open>a \<otimes>\<^sub>o b \<le> a \<otimes>\<^sub>o c\<close>
+proof -
+  have \<open>c - b \<ge> 0\<close>
+    by (simp add: assms(1))
+  with \<open>a \<ge> 0\<close> have \<open>a \<otimes>\<^sub>o (c - b) \<ge> 0\<close>
+    by (intro tensor_op_pos)
+  then have \<open>a \<otimes>\<^sub>o c - a \<otimes>\<^sub>o b \<ge> 0\<close>
+    by (simp add: tensor_op_cbilinear.diff_right)
+  then show ?thesis
+    by simp
+qed
+
+
+lemma tensor_op_mono:
+  fixes a :: \<open>'a ell2 \<Rightarrow>\<^sub>C\<^sub>L 'a ell2\<close> and c :: \<open>'b ell2 \<Rightarrow>\<^sub>C\<^sub>L 'b ell2\<close>
+  assumes \<open>a \<le> b\<close> and \<open>c \<le> d\<close> and \<open>b \<ge> 0\<close> and \<open>c \<ge> 0\<close>
+  shows \<open>a \<otimes>\<^sub>o c \<le> b \<otimes>\<^sub>o d\<close>
+proof -
+  have \<open>a \<otimes>\<^sub>o c \<le> b \<otimes>\<^sub>o c\<close>
+    using \<open>a \<le> b\<close> and \<open>c \<ge> 0\<close>
+    by (rule tensor_op_mono_left)
+  also have \<open>\<dots> \<le> b \<otimes>\<^sub>o d\<close>
+    using \<open>c \<le> d\<close> and \<open>b \<ge> 0\<close>
+    by (rule tensor_op_mono_right)
+  finally show ?thesis
+    by -
+qed
 
 lemma kraus_family_kraus_family_tensor:
   assumes \<open>kraus_family \<EE>\<close> and \<open>kraus_family \<FF>\<close>
   shows \<open>kraus_family (kraus_family_tensor \<EE> \<FF>)\<close>
-  by -
+proof (intro kraus_familyI)
+  from \<open>kraus_family \<EE>\<close>
+  obtain B where B: \<open>(\<Sum>(E, x)\<in>S. E* o\<^sub>C\<^sub>L E) \<le> B\<close> if \<open>finite S\<close> and \<open>S \<subseteq> \<EE>\<close> for S
+    using kraus_family_sums_bounded_by_bound by blast
+  from B[where S=\<open>{}\<close>] have [simp]: \<open>B \<ge> 0\<close>
+    by simp
+  from \<open>kraus_family \<FF>\<close>
+  obtain C where C: \<open>(\<Sum>(F, x)\<in>T. F* o\<^sub>C\<^sub>L F) \<le> C\<close> if \<open>finite T\<close> and \<open>T \<subseteq> \<FF>\<close> for T
+    using kraus_family_sums_bounded_by_bound by blast
+  have \<open>(\<Sum>(G, z)\<in>U. G* o\<^sub>C\<^sub>L G) \<le> B \<otimes>\<^sub>o C\<close> if \<open>finite U\<close> and \<open>U \<subseteq> kraus_family_tensor \<EE> \<FF>\<close> for U
+  proof -
+    define f :: \<open>(('a ell2 \<Rightarrow>\<^sub>C\<^sub>L 'b ell2 \<times> 'c) \<times> 'd ell2 \<Rightarrow>\<^sub>C\<^sub>L 'e ell2 \<times> 'f) \<Rightarrow> _\<close>
+      where \<open>f = (\<lambda>((E,x), (F,y)). (E \<otimes>\<^sub>o F, (E,F,x,y)))\<close>
+    from that
+    obtain V where V_subset: \<open>V \<subseteq> \<EE> \<times> \<FF>\<close> and [simp]: \<open>finite V\<close> and \<open>U = f ` V\<close>
+      apply (simp only: kraus_family_tensor_def flip: f_def)
+      by (meson finite_subset_image)
+    define W where \<open>W = fst ` V \<times> snd ` V\<close>
+    have \<open>inj_on f W\<close>
+      by (auto intro!: inj_onI simp: f_def)
+    from \<open>finite V\<close> have [simp]: \<open>finite W\<close>
+      using W_def by blast
+    have \<open>W \<supseteq> V\<close>
+      by (auto intro!: image_eqI simp: W_def)
+    have \<open>(\<Sum>(G, z)\<in>U. G* o\<^sub>C\<^sub>L G) \<le> (\<Sum>(G, z)\<in>f ` W. G* o\<^sub>C\<^sub>L G)\<close>
+      using \<open>U = f ` V\<close> \<open>V \<subseteq> W\<close>
+      by (auto intro!: sum_mono2 positive_cblinfun_squareI)
+    also have \<open>\<dots> = (\<Sum>((E,x),(F,y))\<in>W. (E \<otimes>\<^sub>o F)* o\<^sub>C\<^sub>L (E \<otimes>\<^sub>o F))\<close>
+      apply (subst sum.reindex)
+      using \<open>inj_on f W\<close>
+      by (auto simp: case_prod_unfold f_def)
+    also have \<open>\<dots> = (\<Sum>((E,x),(F,y))\<in>W. (E* o\<^sub>C\<^sub>L E) \<otimes>\<^sub>o (F* o\<^sub>C\<^sub>L F))\<close>
+      by (simp add: comp_tensor_op tensor_op_adjoint)
+    also have \<open>\<dots> = (\<Sum>(E,x)\<in>fst`V. E* o\<^sub>C\<^sub>L E) \<otimes>\<^sub>o (\<Sum>(F,y)\<in>snd`V. F* o\<^sub>C\<^sub>L F)\<close>
+      unfolding W_def
+      apply (subst sum.Sigma[symmetric])
+        apply (auto intro!: simp: case_prod_beta)
+      by (metis (mono_tags, lifting) sum.cong tensor_op_cbilinear.sum_left tensor_op_cbilinear.sum_right)
+    also have \<open>\<dots> \<le> B \<otimes>\<^sub>o C\<close>
+      using V_subset
+      by (auto intro!: tensor_op_mono B C sum_nonneg intro: positive_cblinfun_squareI)
+    finally show ?thesis
+      by-
+  qed
+  then show \<open>bdd_above ((\<lambda>F. \<Sum>(E, x)\<in>F. E* o\<^sub>C\<^sub>L E) ` {F. finite F \<and> F \<subseteq> kraus_family_tensor \<EE> \<FF>})\<close>
+    by fast
+qed
+
+lemma sandwich_tc_tensor: \<open>sandwich_tc (E \<otimes>\<^sub>o F) (tc_tensor t u) = tc_tensor (sandwich_tc E t) (sandwich_tc F u)\<close>
+  apply (transfer fixing: E F)
+  by (simp add: sandwich_tensor_op)
+
+lemma kraus_family_map_tensor:
+  assumes \<open>kraus_family \<EE>\<close> and \<open>kraus_family \<FF>\<close>
+  shows \<open>kraus_family_map (kraus_family_tensor \<EE> \<FF>) (tc_tensor \<rho> \<sigma>) = tc_tensor (kraus_family_map \<EE> \<rho>) (kraus_family_map \<FF> \<sigma>)\<close>
+proof -
+  have inj: \<open>inj_on (\<lambda>((E, x), F, y). (E \<otimes>\<^sub>o F, E, F, x, y)) (\<EE> \<times> \<FF>)\<close>
+    by (auto intro!: inj_onI)
+  have [simp]: \<open>bounded_linear (\<lambda>x. tc_tensor x (kraus_family_map \<FF> \<sigma>))\<close>
+    by (intro bounded_linear_intros)
+  have [simp]: \<open>bounded_linear (tc_tensor (sandwich_tc E \<rho>))\<close> for E
+    by (intro bounded_linear_intros)
+  have sum2: \<open>(\<lambda>(E, x). sandwich_tc E \<rho>) summable_on \<EE>\<close>
+    using assms(1) kraus_family_map_summable by blast
+  have sum3: \<open>(\<lambda>(F, y). sandwich_tc F \<sigma>) summable_on \<FF>\<close>
+    using assms(2) kraus_family_map_summable by blast
+
+  have \<open>kraus_family (kraus_family_tensor \<EE> \<FF>)\<close>
+    by (simp add: assms kraus_family_kraus_family_tensor)
+  from this[THEN kraus_family_map_summable]
+  have sum1: \<open>(\<lambda>((E, x), F, y). sandwich_tc (E \<otimes>\<^sub>o F) (tc_tensor \<rho> \<sigma>)) summable_on \<EE> \<times> \<FF>\<close>
+    apply (simp add: kraus_family_map_def kraus_family_tensor_def summable_on_reindex inj o_def)
+    by (simp add: case_prod_unfold)
+
+
+  have \<open>kraus_family_map (kraus_family_tensor \<EE> \<FF>) (tc_tensor \<rho> \<sigma>)
+      = (\<Sum>\<^sub>\<infinity>((E,x),(F,y))\<in>\<EE> \<times> \<FF>. sandwich_tc (E \<otimes>\<^sub>o F) (tc_tensor \<rho> \<sigma>))\<close>
+    apply (simp add: kraus_family_map_def kraus_family_tensor_def infsum_reindex inj o_def)
+    by (simp add: case_prod_unfold)
+  also have \<open>\<dots> = (\<Sum>\<^sub>\<infinity>(E,x)\<in>\<EE>. \<Sum>\<^sub>\<infinity>(F,y)\<in>\<FF>. sandwich_tc (E \<otimes>\<^sub>o F) (tc_tensor \<rho> \<sigma>))\<close>
+    apply (subst infsum_Sigma_banach[symmetric])
+    using sum1 by (auto intro!: simp: case_prod_unfold)
+  also have \<open>\<dots> = (\<Sum>\<^sub>\<infinity>(E,x)\<in>\<EE>. \<Sum>\<^sub>\<infinity>(F,y)\<in>\<FF>. tc_tensor (sandwich_tc E \<rho>) (sandwich_tc F \<sigma>))\<close>
+    by (simp add: sandwich_tc_tensor)
+  also have \<open>\<dots> = (\<Sum>\<^sub>\<infinity>(E,x)\<in>\<EE>. tc_tensor (sandwich_tc E \<rho>) (\<Sum>\<^sub>\<infinity>(F,y)\<in>\<FF>. (sandwich_tc F \<sigma>)))\<close>
+    apply (subst infsum_bounded_linear[where f=\<open>tc_tensor (sandwich_tc _ \<rho>)\<close>, symmetric])
+      apply (auto intro!: sum3)[2]
+    by (simp add: o_def case_prod_unfold)
+  also have \<open>\<dots> = (\<Sum>\<^sub>\<infinity>(E,x)\<in>\<EE>. tc_tensor (sandwich_tc E \<rho>) (kraus_family_map \<FF> \<sigma>))\<close>
+    by (simp add: kraus_family_map_def case_prod_unfold)
+  also have \<open>\<dots> = tc_tensor (\<Sum>\<^sub>\<infinity>(E,x)\<in>\<EE>. sandwich_tc E \<rho>) (kraus_family_map \<FF> \<sigma>)\<close>
+    apply (subst infsum_bounded_linear[where f=\<open>\<lambda>x. tc_tensor x (kraus_family_map \<FF> \<sigma>)\<close>, symmetric])
+      apply (auto intro!: sum2)[2]
+    by (simp add: o_def case_prod_unfold)
+  also have \<open>\<dots> = tc_tensor (kraus_family_map \<EE> \<rho>) (kraus_family_map \<FF> \<sigma>)\<close>
+    by (simp add: kraus_family_map_def case_prod_unfold)
+  finally show ?thesis
+    by -
+qed
+
+
+lemma tensor_tc_butterfly: "tc_tensor (tc_butterfly \<psi> \<psi>') (tc_butterfly \<phi> \<phi>') = tc_butterfly (tensor_ell2 \<psi> \<phi>) (tensor_ell2 \<psi>' \<phi>')"
+  apply (transfer fixing: \<phi> \<phi>' \<psi> \<psi>') by simp
+
+
+definition separating_set :: \<open>(('a \<Rightarrow> 'b) \<Rightarrow> bool) \<Rightarrow> 'a set \<Rightarrow> bool\<close> where
+  \<open>separating_set P S \<longleftrightarrow> (\<forall>f g. P f \<longrightarrow> P g \<longrightarrow> (\<forall>x\<in>S. f x = g x) \<longrightarrow> f = g)\<close>
+
+lemma separating_set_mono: \<open>S \<subseteq> T \<Longrightarrow> separating_set P S \<Longrightarrow> separating_set P T\<close>
+  unfolding separating_set_def by fast
+
+lemma separating_set_UNIV[simp]: \<open>separating_set P UNIV\<close>
+  by (auto intro!: ext simp: separating_set_def)
+
+
+lemma eq_from_separatingI:
+  assumes \<open>separating_set P S\<close>
+  assumes \<open>P f\<close> and \<open>P g\<close>
+  assumes \<open>\<And>x. x \<in> S \<Longrightarrow> f x = g x\<close>
+  shows \<open>f = g\<close>
+  using assms by (simp add: separating_set_def)
+
+lemma cblinfun_eq_from_separatingI:
+  fixes a b :: \<open>'a::complex_normed_vector \<Rightarrow>\<^sub>C\<^sub>L 'b::complex_normed_vector\<close>
+  assumes \<open>separating_set (bounded_clinear :: ('a \<Rightarrow> 'b) \<Rightarrow> bool) S\<close>
+  assumes \<open>\<And>x. x \<in> S \<Longrightarrow> a x = b x\<close>
+  shows \<open>a = b\<close>
+  apply (rule cblinfun_eqI, rule fun_cong[where f=\<open>cblinfun_apply _\<close>])
+  using assms(1) apply (rule eq_from_separatingI)
+  using assms(2) by (auto intro!: bounded_cbilinear_apply_bounded_clinear cblinfun.bounded_cbilinear_axioms simp: )
+
+lemma eq_from_separatingI2:
+  assumes \<open>separating_set P ((\<lambda>(x,y). h x y) ` (S\<times>T))\<close>
+  assumes \<open>P f\<close> and \<open>P g\<close>
+  assumes \<open>\<And>x y. x \<in> S \<Longrightarrow> y \<in> T \<Longrightarrow> f (h x y) = g (h x y)\<close>
+  shows \<open>f = g\<close>
+  apply (rule eq_from_separatingI[OF assms(1)])
+  using assms(2-4) by auto
+
+lemma cblinfun_eq_from_separatingI2:
+  fixes a b :: \<open>'a::complex_normed_vector \<Rightarrow>\<^sub>C\<^sub>L 'b::complex_normed_vector\<close>
+  assumes \<open>separating_set (bounded_clinear :: ('a \<Rightarrow> 'b) \<Rightarrow> bool) ((\<lambda>(x,y). h x y) ` (S\<times>T))\<close>
+  assumes \<open>\<And>x y. x \<in> S \<Longrightarrow> y \<in> T \<Longrightarrow> a (h x y) = b (h x y)\<close>
+  shows \<open>a = b\<close>
+  apply (rule cblinfun_eqI, rule fun_cong[where f=\<open>cblinfun_apply _\<close>])
+  using assms(1) apply (rule eq_from_separatingI2)
+  using assms(2) by (auto intro!: bounded_cbilinear_apply_bounded_clinear cblinfun.bounded_cbilinear_axioms simp: )
+
+
+(* lemma separating_set_bounded_clinear_tc_tensor_basis:
+  assumes \<open>ccspan A = \<top>\<close> \<open>ccspan B = \<top>\<close> \<open>ccspan C = \<top>\<close> \<open>ccspan D = \<top>\<close>
+  shows \<open>separating_set bounded_clinear ((\<lambda>(a,b,c,d). tc_tensor (tc_butterfly a b) (tc_butterfly c d)) ` (A\<times>B\<times>C\<times>D))\<close>
+  by - *)
+
+lemma separating_set_bounded_clinear_dense:
+  assumes \<open>ccspan S = \<top>\<close>
+  shows \<open>separating_set bounded_clinear S\<close>
+  using assms
+  apply (auto intro!: ext simp: separating_set_def)
+  apply (rule bounded_clinear_eq_on_closure[where G=S])
+  apply auto
+  using ccspan.rep_eq by force
+
+
+lemma separating_set_bounded_clinear_tc_tensor:
+  shows \<open>separating_set bounded_clinear ((\<lambda>(\<rho>,\<sigma>). tc_tensor \<rho> \<sigma>) ` (UNIV \<times> UNIV))\<close>
+proof -
+  have \<open>\<top> = ccspan ((\<lambda>(x, y). tc_butterfly x y) ` (range ket \<times> range ket))\<close>
+    by (simp add: onb_butterflies_span_trace_class)
+  also have \<open>\<dots> = ccspan ((\<lambda>(x, y, z, w). tc_butterfly (x \<otimes>\<^sub>s y) (z \<otimes>\<^sub>s w)) ` (range ket \<times> range ket \<times> range ket \<times> range ket))\<close>
+    by (auto intro!: arg_cong[where f=ccspan] image_eqI simp: tensor_ell2_ket)
+  also have \<open>\<dots> = ccspan ((\<lambda>(x, y, z, w). tc_tensor (tc_butterfly x z) (tc_butterfly y w)) ` (range ket \<times> range ket \<times> range ket \<times> range ket))\<close>
+    by (simp add: tensor_tc_butterfly)
+  also have \<open>\<dots> \<le> ccspan ((\<lambda>(\<rho>, \<sigma>). tc_tensor \<rho> \<sigma>) ` (UNIV \<times> UNIV))\<close>
+    by (auto intro!: ccspan_mono)
+  finally show ?thesis
+    apply (rule_tac separating_set_bounded_clinear_dense)
+    using top_le by blast
+qed
+
+lemma separating_setI:
+  assumes \<open>\<And>f g. P f \<Longrightarrow> P g \<Longrightarrow> (\<And>x. x\<in>S \<Longrightarrow> f x = g x) \<Longrightarrow> f = g\<close>
+  shows \<open>separating_set P S\<close>
+  by (simp add: assms separating_set_def)
+
+lemma separating_set_bounded_cbilinear_nested:
+  assumes \<open>separating_set (bounded_clinear :: (_ => 'e::complex_normed_vector) \<Rightarrow> _) ((\<lambda>(x, y). h x y) ` (UNIV \<times> UNIV))\<close>
+  assumes \<open>bounded_cbilinear h\<close>
+  assumes \<open>separating_set (bounded_clinear :: (_ => 'e) \<Rightarrow> _) A\<close>
+  assumes \<open>separating_set (bounded_clinear :: (_ => 'e) \<Rightarrow> _) B\<close>
+  shows \<open>separating_set (bounded_clinear :: (_ => 'e) \<Rightarrow> _) ((\<lambda>(x,y). h x y) ` (A \<times> B))\<close>
+proof (rule separating_setI)
+  fix f g :: \<open>'a \<Rightarrow> 'e\<close>
+  assume [simp]: \<open>bounded_clinear f\<close> \<open>bounded_clinear g\<close>
+  have [simp]: \<open>bounded_clinear (\<lambda>x. f (h x y))\<close> for y
+    apply (rule bounded_clinear_compose[OF \<open>bounded_clinear f\<close>])
+    using assms(2) by (rule bounded_cbilinear.bounded_clinear_left)
+  have [simp]: \<open>bounded_clinear (\<lambda>x. g (h x y))\<close> for y
+    apply (rule bounded_clinear_compose[OF \<open>bounded_clinear g\<close>])
+    using assms(2) by (rule bounded_cbilinear.bounded_clinear_left)
+  have [simp]: \<open>bounded_clinear (\<lambda>y. f (h x y))\<close> for x
+    apply (rule bounded_clinear_compose[OF \<open>bounded_clinear f\<close>])
+    using assms(2) by (rule bounded_cbilinear.bounded_clinear_right)
+  have [simp]: \<open>bounded_clinear (\<lambda>y. g (h x y))\<close> for x
+    apply (rule bounded_clinear_compose[OF \<open>bounded_clinear g\<close>])
+    using assms(2) by (rule bounded_cbilinear.bounded_clinear_right)
+
+  assume \<open>z \<in> (\<lambda>(x, y). h x y) ` (A \<times> B) \<Longrightarrow> f z = g z\<close> for z
+  then have \<open>f (h x y) = g (h x y)\<close> if \<open>x \<in> A\<close> and \<open>y \<in> B\<close> for x y
+    using that by auto
+  then have \<open>(\<lambda>x. f (h x y)) = (\<lambda>x. g (h x y))\<close> if \<open>y \<in> B\<close> for y
+    apply (rule_tac eq_from_separatingI[OF assms(3)])
+    using that by auto
+  then have \<open>(\<lambda>y. f (h x y)) = (\<lambda>y. g (h x y))\<close> for x
+    apply (rule_tac eq_from_separatingI[OF assms(4)])
+    apply auto by meson
+  then have \<open>f (h x y) = g (h x y)\<close> for x y
+    by meson
+  with \<open>bounded_clinear f\<close> \<open>bounded_clinear g\<close>
+  show \<open>f = g\<close>
+    apply (rule eq_from_separatingI2[where f=f and g=g and P=bounded_clinear and S=UNIV and T=UNIV, rotated 1])
+    using assms(1) by -
+qed
+
+lemma separating_set_bounded_clinear_antilinear:
+  assumes \<open>separating_set (bounded_clinear :: (_ => 'e::complex_normed_vector conjugate_space) \<Rightarrow> _) A\<close>
+  shows \<open>separating_set (bounded_antilinear :: (_ => 'e) \<Rightarrow> _) A\<close>
+proof (rule separating_setI)
+  fix f g :: \<open>'a \<Rightarrow> 'e\<close>
+  assume \<open>bounded_antilinear f\<close>
+  then have lin_f: \<open>bounded_clinear (to_conjugate_space o f)\<close>
+    by (simp add: bounded_antilinear_o_bounded_antilinear')
+  assume \<open>bounded_antilinear g\<close>
+  then have lin_g: \<open>bounded_clinear (to_conjugate_space o g)\<close>
+    by (simp add: bounded_antilinear_o_bounded_antilinear')
+  assume \<open>f x = g x\<close> if \<open>x \<in> A\<close> for x
+  then have \<open>(to_conjugate_space o f) x = (to_conjugate_space o g) x\<close> if \<open>x \<in> A\<close> for x
+    by (simp add: that)
+  with lin_f lin_g
+  have \<open>to_conjugate_space o f = to_conjugate_space o g\<close>
+    by (rule eq_from_separatingI[OF assms])
+  then show \<open>f = g\<close>
+    by (metis UNIV_I fun.inj_map_strong to_conjugate_space_inverse)
+qed
+
+lemma separating_set_bounded_sesquilinear_nested:
+  assumes \<open>separating_set (bounded_clinear :: (_ => 'e::complex_normed_vector) \<Rightarrow> _) ((\<lambda>(x, y). h x y) ` (UNIV \<times> UNIV))\<close>
+  assumes \<open>bounded_sesquilinear h\<close>
+  assumes sep_A: \<open>separating_set (bounded_clinear :: (_ => 'e conjugate_space) \<Rightarrow> _) A\<close>
+  assumes sep_B: \<open>separating_set (bounded_clinear :: (_ => 'e) \<Rightarrow> _) B\<close>
+  shows \<open>separating_set (bounded_clinear :: (_ => 'e) \<Rightarrow> _) ((\<lambda>(x,y). h x y) ` (A \<times> B))\<close>
+proof (rule separating_setI)
+  fix f g :: \<open>'a \<Rightarrow> 'e\<close>
+  assume [simp]: \<open>bounded_clinear f\<close> \<open>bounded_clinear g\<close>
+  have [simp]: \<open>bounded_antilinear (\<lambda>x. f (h x y))\<close> for y
+    apply (rule bounded_clinear_o_bounded_antilinear[OF \<open>bounded_clinear f\<close>])
+    using assms(2) by (rule bounded_sesquilinear.bounded_antilinear_left)
+  have [simp]: \<open>bounded_antilinear (\<lambda>x. g (h x y))\<close> for y
+    apply (rule bounded_clinear_o_bounded_antilinear[OF \<open>bounded_clinear g\<close>])
+    using assms(2) by (rule bounded_sesquilinear.bounded_antilinear_left)
+  have [simp]: \<open>bounded_clinear (\<lambda>y. f (h x y))\<close> for x
+    apply (rule bounded_clinear_compose[OF \<open>bounded_clinear f\<close>])
+    using assms(2) by (rule bounded_sesquilinear.bounded_clinear_right)
+  have [simp]: \<open>bounded_clinear (\<lambda>y. g (h x y))\<close> for x
+    apply (rule bounded_clinear_compose[OF \<open>bounded_clinear g\<close>])
+    using assms(2) by (rule bounded_sesquilinear.bounded_clinear_right)
+
+  from sep_A have sep_A': \<open>separating_set (bounded_antilinear :: (_ => 'e) \<Rightarrow> _) A\<close>
+    by (rule separating_set_bounded_clinear_antilinear)
+  assume \<open>z \<in> (\<lambda>(x, y). h x y) ` (A \<times> B) \<Longrightarrow> f z = g z\<close> for z
+  then have \<open>f (h x y) = g (h x y)\<close> if \<open>x \<in> A\<close> and \<open>y \<in> B\<close> for x y
+    using that by auto
+  then have \<open>(\<lambda>x. f (h x y)) = (\<lambda>x. g (h x y))\<close> if \<open>y \<in> B\<close> for y
+    apply (rule_tac eq_from_separatingI[OF sep_A'])
+    using that by auto
+  then have \<open>(\<lambda>y. f (h x y)) = (\<lambda>y. g (h x y))\<close> for x
+    apply (rule_tac eq_from_separatingI[OF sep_B])
+    apply auto by meson
+  then have \<open>f (h x y) = g (h x y)\<close> for x y
+    by meson
+  with \<open>bounded_clinear f\<close> \<open>bounded_clinear g\<close>
+  show \<open>f = g\<close>
+    apply (rule eq_from_separatingI2[where f=f and g=g and P=bounded_clinear and S=UNIV and T=UNIV, rotated 1])
+    using assms(1) by -
+qed
+
+
+(* TODO generalize: this just needs that tc_tensor is bounded_bilinear *)
+lemma separating_set_bounded_clinear_tc_tensor_nested:
+  assumes \<open>separating_set (bounded_clinear :: (_ => 'e::complex_normed_vector) \<Rightarrow> _) A\<close>
+  assumes \<open>separating_set (bounded_clinear :: (_ => 'e::complex_normed_vector) \<Rightarrow> _) B\<close>
+  shows \<open>separating_set (bounded_clinear :: (_ => 'e::complex_normed_vector) \<Rightarrow> _) ((\<lambda>(\<rho>,\<sigma>). tc_tensor \<rho> \<sigma>) ` (A \<times> B))\<close>
+  using separating_set_bounded_clinear_tc_tensor bounded_cbilinear_tc_tensor assms
+  by (rule separating_set_bounded_cbilinear_nested)
+(* proof (rule separating_setI)
+  fix f g :: \<open>(('a \<times> 'c) ell2, ('b \<times> 'd) ell2) trace_class \<Rightarrow> 'e\<close>
+  assume [simp]: \<open>bounded_clinear f\<close> \<open>bounded_clinear g\<close>
+  have [simp]: \<open>bounded_clinear (\<lambda>\<rho>. f (tc_tensor \<rho> \<sigma>))\<close> for \<sigma>
+    by -
+  have [simp]: \<open>bounded_clinear (\<lambda>\<rho>. g (tc_tensor \<rho> \<sigma>))\<close> for \<sigma>
+    by -
+  have [simp]: \<open>bounded_clinear (\<lambda>\<sigma>. f (tc_tensor \<rho> \<sigma>))\<close> for \<rho>
+    by -
+  have [simp]: \<open>bounded_clinear (\<lambda>\<sigma>. g (tc_tensor \<rho> \<sigma>))\<close> for \<rho>
+    by -
+
+  assume \<open>x \<in> (\<lambda>(\<rho>, \<sigma>). tc_tensor \<rho> \<sigma>) ` (A \<times> B) \<Longrightarrow> f x = g x\<close> for x
+  then have \<open>f (tc_tensor \<rho> \<sigma>) = g (tc_tensor \<rho> \<sigma>)\<close> if \<open>\<rho> \<in> A\<close> and \<open>\<sigma> \<in> B\<close> for \<rho> \<sigma>
+    using that by auto
+  then have \<open>(\<lambda>\<rho>. f (tc_tensor \<rho> \<sigma>)) = (\<lambda>\<rho>. g (tc_tensor \<rho> \<sigma>))\<close> if \<open>\<sigma> \<in> B\<close> for \<sigma>
+    apply (rule eq_from_separatingI[OF assms(1), rotated -1])
+    using that by auto
+  then have \<open>(\<lambda>\<sigma>. f (tc_tensor \<rho> \<sigma>)) = (\<lambda>\<sigma>. g (tc_tensor \<rho> \<sigma>))\<close> for \<rho>
+    apply (rule_tac eq_from_separatingI[OF assms(2)])
+    apply auto by meson
+  then have \<open>f (tc_tensor \<rho> \<sigma>) = g (tc_tensor \<rho> \<sigma>)\<close> for \<rho> \<sigma>
+    by meson
+  with \<open>bounded_clinear f\<close> \<open>bounded_clinear g\<close>
+  show \<open>f = g\<close>
+    by (rule eq_from_separatingI2[OF separating_set_bounded_clinear_tc_tensor])
+qed *)
+
+
+lemma bounded_sesquilinear_tc_butterfly[iff]: \<open>bounded_sesquilinear (\<lambda>a b. tc_butterfly b a)\<close>
+  by (auto intro!: bounded_sesquilinear.intro exI[of _ 1]
+      simp: tc_butterfly_add_left tc_butterfly_add_right norm_tc_butterfly)
+
+lemma separating_set_tc_butterfly: \<open>separating_set bounded_clinear ((\<lambda>(g,h). tc_butterfly g h) ` (UNIV \<times> UNIV))\<close>
+  apply (rule separating_set_mono[where S=\<open>(\<lambda>(g, h). tc_butterfly g h) ` (some_chilbert_basis \<times> some_chilbert_basis)\<close>])
+  by (auto intro!: separating_set_bounded_clinear_dense onb_butterflies_span_trace_class) 
+
+lemma separating_set_tc_butterfly_nested:
+  assumes \<open>separating_set (bounded_clinear :: (_ \<Rightarrow> 'c::complex_normed_vector) \<Rightarrow> _) A\<close>
+  assumes \<open>separating_set (bounded_clinear :: (_ \<Rightarrow> 'c conjugate_space) \<Rightarrow> _) B\<close>
+  shows \<open>separating_set (bounded_clinear :: (_ \<Rightarrow> 'c) \<Rightarrow> _) ((\<lambda>(g,h). tc_butterfly g h) ` (A \<times> B))\<close>
+proof -
+  from separating_set_tc_butterfly
+  have \<open>separating_set bounded_clinear ((\<lambda>(g,h). tc_butterfly g h) ` prod.swap ` (UNIV \<times> UNIV))\<close>
+    by simp
+  then have \<open>separating_set bounded_clinear ((\<lambda>(g,h). tc_butterfly h g) ` (UNIV \<times> UNIV))\<close>
+    unfolding image_image by simp
+  then have \<open>separating_set (bounded_clinear :: (_ \<Rightarrow> 'c) \<Rightarrow> _) ((\<lambda>(g,h). tc_butterfly h g) ` (B \<times> A))\<close>
+    apply (rule separating_set_bounded_sesquilinear_nested)
+    apply (rule bounded_sesquilinear_tc_butterfly)
+    using assms by auto
+  then have \<open>separating_set (bounded_clinear :: (_ \<Rightarrow> 'c) \<Rightarrow> _) ((\<lambda>(g,h). tc_butterfly h g) ` prod.swap ` (A \<times> B))\<close>
+    by (smt (verit, del_insts) SigmaE SigmaI eq_from_separatingI image_iff pair_in_swap_image separating_setI)
+  then show ?thesis
+    unfolding image_image by simp
+qed
+
+(* proof (rule separating_setI)
+  fix f g :: \<open>('b, 'a) trace_class \<Rightarrow> 'c\<close>
+  assume [simp]: \<open>bounded_clinear f\<close> \<open>bounded_clinear g\<close>
+  have [simp]: \<open>bounded_clinear (\<lambda>\<rho>. f (tc_butterfly \<rho> \<sigma>))\<close> for \<sigma>
+try0
+sledgehammer [dont_slice]
+by -
+  have [simp]: \<open>bounded_clinear (\<lambda>\<rho>. g (tc_butterfly \<rho> \<sigma>))\<close> for \<sigma>
+try0
+sledgehammer [dont_slice]
+by -
+  have [simp]: \<open>bounded_clinear (\<lambda>\<sigma>. f (tc_butterfly \<rho> \<sigma>))\<close> for \<rho>
+try0
+sledgehammer [dont_slice]
+by -
+  have [simp]: \<open>bounded_clinear (\<lambda>\<sigma>. g (tc_butterfly \<rho> \<sigma>))\<close> for \<rho>
+try0
+sledgehammer [dont_slice]
+by -
+
+  assume \<open>x \<in> (\<lambda>(g, h). tc_butterfly g h) ` (A \<times> B) \<Longrightarrow> f x = g x\<close> for x
+  then have \<open>f (tc_butterfly \<rho> \<sigma>) = g (tc_butterfly \<rho> \<sigma>)\<close> if \<open>\<rho> \<in> A\<close> and \<open>\<sigma> \<in> B\<close> for \<rho> \<sigma>
+    using that by auto
+  then have \<open>(\<lambda>\<rho>. f (tc_butterfly \<rho> \<sigma>)) = (\<lambda>\<rho>. g (tc_butterfly \<rho> \<sigma>))\<close> if \<open>\<sigma> \<in> B\<close> for \<sigma>
+    apply (rule eq_from_separatingI[OF assms(1), rotated -1])
+    using that by auto
+  then have \<open>(\<lambda>\<sigma>. f (tc_butterfly \<rho> \<sigma>)) = (\<lambda>\<sigma>. g (tc_butterfly \<rho> \<sigma>))\<close> for \<rho>
+    apply (rule_tac eq_from_separatingI[OF assms(2)])
+    apply auto by meson
+  then have \<open>f (tc_butterfly \<rho> \<sigma>) = g (tc_butterfly \<rho> \<sigma>)\<close> for \<rho> \<sigma>
+    by meson
+  with \<open>bounded_clinear f\<close> \<open>bounded_clinear g\<close>
+  show \<open>f = g\<close>
+    by (rule eq_from_separatingI2[OF separating_set_tc_butterfly])
+qed *)
+
 
 lemma kraus_tensor_cong:
   assumes \<open>kraus_equivalent \<EE> \<EE>'\<close>
   assumes \<open>kraus_equivalent \<FF> \<FF>'\<close>
   shows \<open>kraus_equivalent (kraus_family_tensor \<EE> \<FF>) (kraus_family_tensor \<EE>' \<FF>')\<close>
-  by -
-
-
-lemma onb_butterflies_span_trace_class:
-  fixes A B :: \<open>'a::chilbert_space set\<close>
-  assumes \<open>is_onb A\<close> and \<open>is_onb B\<close>
-  shows \<open>ccspan ((\<lambda>(x, y). tc_butterfly x y) ` (A\<times>B)) = \<top>\<close>
-proof -
-  have \<open>closure (cspan ((\<lambda>(x, y). tc_butterfly x y) ` (A\<times>B))) \<supseteq> Collect rank1_tc\<close>
-    by -
-  moreover have \<open>cspan (Collect rank1_tc) = Collect finite_rank_tc\<close>
-    using finite_rank_tc_def' by fastforce
-  moreover have \<open>closure (Collect finite_rank_tc :: ('a,'a) trace_class set) = UNIV\<close>
-    by (rule finite_rank_tc_dense)
-  ultimately have \<open>closure (cspan ((\<lambda>(x, y). tc_butterfly x y) ` (A\<times>B))) \<supseteq> UNIV\<close>
-    by (smt (verit, ccfv_SIG) closure_closure closure_is_csubspace closure_mono complex_vector.span_minimal complex_vector.subspace_span)
-  then show ?thesis
-    by (metis ccspan.abs_eq ccspan_UNIV closure_UNIV complex_vector.span_UNIV top.extremum_uniqueI)
+proof (intro kraus_equivalent_def[THEN iffD2] conjI)
+  have [iff]: \<open>kraus_family \<EE>\<close> \<open>kraus_family \<FF>\<close>
+    using assms kraus_equivalent_def by auto
+  then show family_\<EE>\<FF>: \<open>kraus_family (kraus_family_tensor \<EE> \<FF>)\<close>
+    by (simp add: kraus_family_kraus_family_tensor)
+  have [iff]: \<open>kraus_family \<EE>'\<close> \<open>kraus_family \<FF>'\<close>
+    using assms kraus_equivalent_def by auto
+  then show family_\<EE>'\<FF>': \<open>kraus_family (kraus_family_tensor \<EE>' \<FF>')\<close>
+    by (simp add: kraus_family_kraus_family_tensor)
+  show \<open>kraus_family_map (kraus_family_tensor \<EE> \<FF>) = kraus_family_map (kraus_family_tensor \<EE>' \<FF>')\<close>
+  proof (rule eq_from_separatingI2[OF separating_set_bounded_clinear_tc_tensor])
+    show \<open>bounded_clinear (kraus_family_map (kraus_family_tensor \<EE> \<FF>))\<close>
+      by (simp add: family_\<EE>\<FF> kraus_family_map_bounded_clinear)
+    show \<open>bounded_clinear (kraus_family_map (kraus_family_tensor \<EE>' \<FF>'))\<close>
+      by (simp add: family_\<EE>'\<FF>' kraus_family_map_bounded_clinear)
+    have \<EE>\<EE>': \<open>kraus_family_map \<EE> \<rho> = kraus_family_map \<EE>' \<rho>\<close> for \<rho>
+      by (metis assms(1) kraus_equivalent_def)
+    have \<FF>\<FF>': \<open>kraus_family_map \<FF> \<rho> = kraus_family_map \<FF>' \<rho>\<close> for \<rho>
+      by (metis assms(2) kraus_equivalent_def)
+    fix \<rho> :: \<open>('a ell2, 'a ell2) trace_class\<close> and \<sigma> :: \<open>('e ell2, 'e ell2) trace_class\<close>
+    show \<open>kraus_family_map (kraus_family_tensor \<EE> \<FF>) (tc_tensor \<rho> \<sigma>) = kraus_family_map (kraus_family_tensor \<EE>' \<FF>') (tc_tensor \<rho> \<sigma>)\<close>
+      by (auto intro!: simp: kraus_family_map_tensor \<EE>\<EE>' \<FF>\<FF>'
+          simp flip: tensor_ell2_ket tensor_tc_butterfly)
+  qed
 qed
 
 lift_definition kraus_map_tensor :: \<open>('a ell2, 'b ell2) kraus_map \<Rightarrow> ('c ell2, 'd ell2) kraus_map \<Rightarrow> (('a\<times>'c) ell2, ('b\<times>'d) ell2) kraus_map\<close> is
   \<open>\<lambda>\<EE> \<FF>. kraus_family_flatten (kraus_family_tensor \<EE> \<FF>)\<close>
   by (intro kraus_equivalent_kraus_family_flatten_left kraus_equivalent_kraus_family_flatten_right kraus_tensor_cong)
 
-(* 
+lemma kraus_map_tensor:
+  shows \<open>kraus_map_apply (kraus_map_tensor \<EE> \<FF>) (tc_tensor \<rho> \<sigma>) = tc_tensor (kraus_map_apply \<EE> \<rho>) (kraus_map_apply \<FF> \<sigma>)\<close>
+  apply (transfer fixing: \<rho> \<sigma>)
+  by (simp add: kraus_equivalent_def kraus_family_flatten_same_map kraus_family_kraus_family_tensor kraus_family_map_tensor)
 
-TODO:
-* kraus_family (kraus_family_tensor \<dots>)
-* kraus_map_apply (kraus_map_tensor \<EE> \<FF>) (tensor_tc \<rho> \<sigma>)) = \<dots>
-* kraus_map_tensor kraus_map_id kraus_map_trace = partial_trace
-* kraus_map_tensor of compositions
-* partial_trace ((kraus_map_tensor id \<EE>) \<rho>) = partial_trace \<rho>  if  trace_preserving \<EE>
+lemma kraus_map_tensor_compose_distribute:
+  shows \<open>kraus_map_tensor (kraus_map_comp \<EE> \<FF>) (kraus_map_comp \<GG> \<HH>) = kraus_map_comp (kraus_map_tensor \<EE> \<GG>) (kraus_map_tensor \<FF> \<HH>)\<close>
+  apply (intro kraus_map_apply_inj cblinfun_apply_inject[THEN iffD1] eq_from_separatingI2[OF separating_set_bounded_clinear_tc_tensor])
+  by (auto intro!: cblinfun.bounded_clinear_right simp: kraus_map_tensor kraus_map_apply_comp)
 
-*)
+(* definition kraus_family_trace :: \<open>('a::chilbert_space, 'b::one_dim, 'a) kraus_family\<close> where
+  \<open>kraus_family_trace = (\<lambda>b. (vector_to_cblinfun b*, b)) ` some_chilbert_basis\<close>
+
+lemma kraus_family_trace[iff]: \<open>kraus_family (kraus_family_trace :: ('a::chilbert_space, 'b::one_dim, 'a) kraus_family)\<close>
+proof (intro kraus_familyI bdd_aboveI)
+  fix M assume \<open>M \<in> (\<lambda>F. \<Sum>(E :: 'a \<Rightarrow>\<^sub>C\<^sub>L 'b, x)\<in>F. E* o\<^sub>C\<^sub>L E) ` {F. finite F \<and> F \<subseteq> kraus_family_trace}\<close>
+  then obtain F where M_sum: \<open>M = (\<Sum>(E :: 'a \<Rightarrow>\<^sub>C\<^sub>L 'b, x)\<in>F. E* o\<^sub>C\<^sub>L E)\<close> and \<open>finite F\<close> and \<open>F \<subseteq> kraus_family_trace\<close>
+    by blast
+  define F' where \<open>F' = snd ` F\<close>
+  from \<open>F \<subseteq> kraus_family_trace\<close>
+  have \<open>inj_on snd F\<close>
+    apply (auto intro!: inj_onI simp: kraus_family_trace_def)
+    using subsetD by fastforce
+  from \<open>F \<subseteq> kraus_family_trace\<close>
+  have ortho_F': \<open>is_ortho_set F'\<close>
+    apply (auto intro!: simp: F'_def kraus_family_trace_def image_image elim!: subset_imageE)
+    using is_ortho_set_antimono is_ortho_set_some_chilbert_basis by blast
+  from \<open>F \<subseteq> kraus_family_trace\<close>
+  have norm_F': \<open>b \<in> F' \<Longrightarrow> norm b = 1\<close> for b
+    apply (auto intro!: simp: F'_def kraus_family_trace_def image_image elim!: subset_imageE)
+    using is_normal_some_chilbert_basis by blast
+  have \<open>a* o\<^sub>C\<^sub>L a = (vector_to_cblinfun b* )* o\<^sub>C\<^sub>L (vector_to_cblinfun b* :: _ \<Rightarrow>\<^sub>C\<^sub>L 'b)\<close> if \<open>(a,b) \<in> F\<close> for a b
+    using \<open>F \<subseteq> kraus_family_trace\<close> that
+    by (simp add: kraus_family_trace_def subset_iff image_def)
+  then have \<open>M = (\<Sum>b\<in>F'. vector_to_cblinfun b o\<^sub>C\<^sub>L (vector_to_cblinfun b* :: _ \<Rightarrow>\<^sub>C\<^sub>L 'b))\<close>
+    by (auto intro!: sum.cong simp: M_sum F'_def sum.reindex \<open>inj_on snd F\<close>)
+  then have \<open>M = (\<Sum>b\<in>F'. butterfly b b)\<close>
+    by (metis (mono_tags, lifting) Finite_Cartesian_Product.sum_cong_aux butterfly_def_one_dim)
+  also from ortho_F' norm_F' have \<open>\<dots> \<le> id_cblinfun\<close>
+    by (rule sum_butterfly_leq_id)
+  finally show \<open>M \<le> id_cblinfun\<close>
+    by -
+qed *)
+
+lemma infsum_bounded_linear_invertible:
+  assumes \<open>bounded_linear f\<close>
+  assumes \<open>bounded_linear f'\<close>
+  assumes \<open>f' o f = id\<close>
+  shows \<open>infsum (f \<circ> g) S = f (infsum g S)\<close>
+proof (cases \<open>g summable_on S\<close>)
+  case True
+  then show ?thesis
+    using assms(1) infsum_bounded_linear by blast
+next
+  case False
+  have \<open>\<not> (f o g) summable_on S\<close>
+  proof (rule ccontr)
+    assume \<open>\<not> \<not> f \<circ> g summable_on S\<close>
+    with \<open>bounded_linear f'\<close> have \<open>f' o f o g summable_on S\<close>
+      by (auto intro: summable_on_bounded_linear simp: o_def)
+    then have \<open>g summable_on S\<close>
+      by (simp add: assms(3))
+    with False show False
+      by blast
+  qed
+  then show ?thesis
+    by (simp add: False assms(1) infsum_not_exists linear_simps(3))
+qed
+
+
+(* lemma kraus_family_map_trace: \<open>trace_tc t = one_dim_iso (kraus_family_map (kraus_family_trace :: ('a::chilbert_space, 'b::one_dim, 'a) kraus_family) t)\<close>
+proof -
+  note infsum_one_dim = infsum_bounded_linear_invertible[symmetric, OF 
+      bounded_clinear.bounded_linear[OF bounded_clinear_one_dim_iso]
+      bounded_clinear.bounded_linear[OF bounded_clinear_one_dim_iso]]
+  have \<open>(one_dim_iso (kraus_family_map (kraus_family_trace :: ('a::chilbert_space, 'b::one_dim, 'a) kraus_family) t) :: complex) = 
+      (\<Sum>\<^sub>\<infinity>x\<in>some_chilbert_basis. one_dim_iso (from_trace_class (sandwich_tc (vector_to_cblinfun x* :: _ \<Rightarrow>\<^sub>C\<^sub>L 'b) *\<^sub>V t)))\<close>
+    apply (simp add: kraus_family_map_def kraus_family_trace_def infsum_reindex inj_on_def o_def trace_tc.rep_eq)
+    apply (subst infsum_one_dim)
+    by (auto simp: o_def)
+  also have \<open>\<dots> = (\<Sum>\<^sub>\<infinity>x\<in>some_chilbert_basis. x \<bullet>\<^sub>C (from_trace_class t *\<^sub>V x))\<close>
+    apply (simp only: from_trace_class_sandwich_tc sandwich_apply)
+    by simp
+  also have \<open>\<dots> = trace_tc t\<close>
+    by (simp add: infsum_reindex inj_on_def o_def trace_tc.rep_eq trace_alt_def[OF is_onb_some_chilbert_basis])
+  finally show ?thesis
+    by simp
+qed *)
+
+(* lift_definition kraus_map_trace :: \<open>('a::chilbert_space, 'b::one_dim) kraus_map\<close> is \<open>kraus_family_flatten kraus_family_trace\<close>
+  by (auto simp: kraus_equivalent_def) *)
+
+lemma trace_kraus_map_is_trace': \<open>trace_tc t = one_dim_iso (kraus_map_apply trace_kraus_map t)\<close>
+  apply (transfer fixing: t)
+  by (simp add: kraus_family_flatten_same_map trace_kraus_family_is_kraus_family trace_kraus_family_is_trace)
+
+lemma partial_trace_scaleC: \<open>partial_trace (c *\<^sub>C t) = c *\<^sub>C partial_trace t\<close>
+  by (simp add: partial_trace_def infsum_scaleC_right compose_tcr.scaleC_right compose_tcl.scaleC_left)
+
+lemma partial_trace_tensor: \<open>partial_trace (tc_tensor t u) = trace_tc u *\<^sub>C t\<close>
+proof -
+  define t' u' where \<open>t' = from_trace_class t\<close> and \<open>u' = from_trace_class u\<close>
+  have 1: \<open>(\<lambda>j. ket j \<bullet>\<^sub>C (from_trace_class u *\<^sub>V ket j)) summable_on UNIV\<close>
+    using  trace_exists[where B=\<open>range ket\<close> and A=\<open>from_trace_class u\<close>]
+    by (simp add: summable_on_reindex o_def)
+  have \<open>partial_trace (tc_tensor t u) =
+      (\<Sum>\<^sub>\<infinity>j. compose_tcl (compose_tcr (tensor_ell2_right (ket j)*) (tc_tensor t u)) (tensor_ell2_right (ket j)))\<close>
+    by (simp add: partial_trace_def)
+  also have \<open>\<dots> = (\<Sum>\<^sub>\<infinity>j. (ket j \<bullet>\<^sub>C (from_trace_class u *\<^sub>V ket j)) *\<^sub>C t)\<close>
+  proof -
+    have *: \<open>tensor_ell2_right (ket j)* o\<^sub>C\<^sub>L t' \<otimes>\<^sub>o u' o\<^sub>C\<^sub>L tensor_ell2_right (ket j) =
+         (ket j \<bullet>\<^sub>C (u' *\<^sub>V ket j)) *\<^sub>C t'\<close> for j
+      by (auto intro!: cblinfun_eqI simp: tensor_op_ell2)
+    show ?thesis
+    apply (rule infsum_cong)
+      by (auto intro!: from_trace_class_inject[THEN iffD1] simp flip: t'_def u'_def
+        simp: * compose_tcl.rep_eq compose_tcr.rep_eq tc_tensor.rep_eq scaleC_trace_class.rep_eq)
+  qed
+  also have \<open>\<dots> = trace_tc u *\<^sub>C t\<close>
+    by (auto intro!: infsum_scaleC_left simp: trace_tc_def trace_alt_def[OF is_onb_ket] infsum_reindex o_def 1)
+  finally show ?thesis
+    by -
+qed
+
+
+lemma bounded_clinear_partial_trace[bounded_clinear, iff]: \<open>bounded_clinear partial_trace\<close>
+  apply (rule bounded_clinearI[where K=1])
+  by (auto simp add: partial_trace_plus partial_trace_scaleC partial_trace_norm_reducing)
+
+
+lemma partial_trace_as_kraus_map: \<open>partial_trace t = 
+  kraus_map_apply (kraus_map_of_op (tensor_ell2_right 1*))
+  (kraus_map_apply (kraus_map_tensor kraus_map_id trace_kraus_map) t)\<close>
+(* TODO: also "kraus_map_apply (kraus_map_tensor kraus_map_id kraus_map_trace) t = ... partial_trace ... *)
+proof (rule fun_cong[where x=t], rule eq_from_separatingI2[OF separating_set_bounded_clinear_tc_tensor])
+  show \<open>bounded_clinear partial_trace\<close>
+    by simp
+  show \<open>bounded_clinear
+     (\<lambda>a. kraus_map_apply (kraus_map_of_op (tensor_ell2_right 1*)) *\<^sub>V
+           kraus_map_apply (kraus_map_tensor kraus_map_id trace_kraus_map) *\<^sub>V a)\<close>
+    by (intro bounded_linear_intros)
+  fix \<rho> :: \<open>('a ell2, 'a ell2) trace_class\<close> and \<sigma> :: \<open>('b ell2, 'b ell2) trace_class\<close>
+  show \<open>partial_trace (tc_tensor \<rho> \<sigma>) =
+           kraus_map_apply (kraus_map_of_op (tensor_ell2_right 1*)) *\<^sub>V
+           kraus_map_apply (kraus_map_tensor kraus_map_id trace_kraus_map) *\<^sub>V tc_tensor \<rho> \<sigma>\<close>
+    apply (auto intro!: from_trace_class_inject[THEN iffD1]
+        simp: partial_trace_tensor kraus_map_tensor trace_kraus_map_is_trace kraus_map_of_op_apply
+        from_trace_class_sandwich_tc sandwich_apply trace_tc.rep_eq tc_tensor.rep_eq scaleC_trace_class.rep_eq)
+    by (auto intro!: cblinfun_eqI simp: tensor_op_ell2)
+qed
+
+lemma partial_trace_ignore_trace_preserving_map:
+  assumes \<open>trace_preserving \<EE>\<close>
+  shows \<open>partial_trace (kraus_map_apply (kraus_map_tensor kraus_map_id \<EE>) \<rho>) = partial_trace \<rho>\<close>
+proof (rule fun_cong[where x=\<rho>], rule eq_from_separatingI2[OF separating_set_bounded_clinear_tc_tensor])
+  show \<open>bounded_clinear (\<lambda>a. partial_trace (kraus_map_apply (kraus_map_tensor kraus_map_id \<EE>) *\<^sub>V a))\<close>
+    by (intro bounded_linear_intros)
+  show \<open>bounded_clinear partial_trace\<close>
+    by (intro bounded_linear_intros)
+  fix \<rho> :: \<open>('c ell2, 'c ell2) trace_class\<close> and \<sigma> :: \<open>('a ell2, 'a ell2) trace_class\<close>
+  from assms
+  show \<open>partial_trace (kraus_map_apply (kraus_map_tensor kraus_map_id \<EE>) *\<^sub>V tc_tensor \<rho> \<sigma>) = partial_trace (tc_tensor \<rho> \<sigma>)\<close>
+    by (auto intro!: simp: kraus_map_tensor partial_trace_tensor trace_preserving_def)
+qed
+
+lemma kraus_map_comp_id_left[simp]: \<open>kraus_map_comp kraus_map_id \<EE> = \<EE>\<close>
+  by (auto intro!: kraus_map_apply_inj cblinfun_eqI simp: kraus_map_apply_comp kraus_map_id_apply)
+
+lemma kraus_map_comp_id_right[simp]: \<open>kraus_map_comp \<EE> kraus_map_id = \<EE>\<close>
+  by (auto intro!: kraus_map_apply_inj cblinfun_eqI simp: kraus_map_apply_comp kraus_map_id_apply)
 
 end
